finished an example that calls an unknown adversary sharing a RO copy of a capability

theories/examples/lse.v
@@ -1,844 +1,516 @@
 From iris.algebra Require Import frac.
 From iris.proofmode Require Import tactics.
-Require Import Eqdep_dec.
-From cap_machine Require Import stdpp_extra iris_extra
-     rules logrel fundamental region_invariants
-     region_invariants_revocation region_invariants_static region_invariants_uninitialized. 
-From cap_machine.examples Require Import region_macros stack_macros stack_macros_u stack_macros_helpers scall_u awkward_example_helpers.
-From stdpp Require Import countable.
+Require Import Eqdep_dec List.
+From cap_machine Require Import rules logrel macros_helpers macros fundamental call callback.
 
-Section lse.
-   Context {Σ:gFunctors} {memg:memG Σ} {regg:regG Σ}
-          {stsg : STSG Addr region_type Σ} {heapg : heapG Σ}
-          `{MonRef: MonRefG (leibnizO _) CapR_rtc Σ} {nainv: logrel_na_invs Σ}
+Lemma map_to_list_delete_fst {A B} `{Countable A} (m : gmap A B) (i : A) (x : B) :
+  ∀ l, i :: l ≡ₚ(map_to_list m).*1 ->
+       NoDup (i :: l) →
+       (map_to_list (delete i m)).*1 ≡ₚl.
+Proof.
+  intros l Hl Hdup.
+  assert (i ∈ (map_to_list m).*1) as Hin.
+  { rewrite -Hl. constructor. }
+  apply NoDup_cons_iff in Hdup as [Hnin Hdup]. 
+  apply Permutation.NoDup_Permutation;auto. 
+  apply NoDup_map_to_list_fst. done.
+  set l' := zip l (repeat x (length l)).
+  assert (l = l'.*1) as Heq;[rewrite fst_zip;auto;rewrite repeat_length;lia|]. 
+  intros i0. split.
+  - intros Hinx%elem_of_list_In%elem_of_list_fmap.
+    destruct Hinx as [ [? ?] [? Hinx] ]. simpl in *. subst a.
+    apply elem_of_map_to_list in Hinx.
+    destruct (decide (i = i0));[subst i;rewrite lookup_delete in Hinx;inversion Hinx|].
+    rewrite lookup_delete_ne in Hinx;auto.
+    apply elem_of_map_to_list in Hinx.
+    assert (i0 ∈ (map_to_list m).*1) as Hinx'.
+    { apply elem_of_list_fmap. exists (i0,b). split;auto. }
+    revert Hinx'. rewrite -Hl =>Hinx'. apply elem_of_cons in Hinx' as [Hcontr | Hinx'];[congruence|].
+    apply elem_of_list_In;auto. 
+  - intros Hinx%elem_of_list_In.
+    apply elem_of_list_In. revert Hnin; rewrite -elem_of_list_In => Hnin. 
+    assert (i ≠ i0) as Hne;[congruence|simplify_map_eq].
+    assert (i0 ∈ i :: l) as Hin'.
+    { constructor. auto. }
+    revert Hin'. rewrite Hl =>Hin'.
+    apply map_to_list_fst in Hin' as [x' Hx].
+    apply elem_of_map_to_list in Hx.
+    apply map_to_list_fst. exists x'. apply elem_of_map_to_list.
+    rewrite lookup_delete_ne;auto. 
+Qed.
+
+Lemma big_sepM_to_create_gmap_default {Σ : gFunctors} {A B : Type} `{Countable A} (m m' : gmap A B) (φ : A -> B -> iProp Σ) (b : B) (l : list A) :
+  l ≡ₚ(map_to_list m).*1 →
+  m' = create_gmap_default l b →
+  ([∗ map] a↦_ ∈ m, φ a b) -∗ ([∗ map] a↦b' ∈ m', φ a b').
+Proof.
+  iIntros (Hl Hm) "Hm".
+  iInduction l as [|a l] "IH" forall (m m' Hl Hm). 
+  - simpl in Hm. rewrite Hm. done. 
+  - assert (NoDup (a :: l)) as Hdup.
+    { rewrite Hl. apply NoDup_map_to_list_fst. done. }
+    assert (a ∈ (map_to_list m).*1) as Hin'.
+    { rewrite -Hl. constructor. }
+    assert (is_Some(m !! a)) as [b' Hsome].
+    { apply elem_of_gmap_dom. rewrite -list_to_set_map_to_list. apply elem_of_list_to_set. auto. }
+    iDestruct (big_sepM_delete _ _ a with "Hm") as "[Ha Hm]";eauto.
+    iApply big_sepM_delete;[|iFrame].
+    { rewrite Hm.  apply lookup_insert. }
+    rewrite Hm /= delete_insert_delete.
+    iApply ("IH" $! (delete a m));[..|iFrame]. 
+    + iPureIntro. rewrite map_to_list_delete_fst;eauto. 
+    + iPureIntro. rewrite delete_notin;auto.
+      destruct (create_gmap_default l b !! a) eqn:Hsome';auto. 
+      exfalso. apply NoDup_cons_iff in Hdup as [Hnin Hdup].
+      apply Hnin. apply elem_of_list_In.
+      apply create_gmap_default_lookup_is_Some in Hsome' as [Hin Hsome']. subst.
+      auto. 
+Qed. 
+    
+    
+Section roe.
+  Context {Σ:gFunctors} {memg:memG Σ} {regg:regG Σ}
+          {nainv: logrel_na_invs Σ}
           `{MP: MachineParameters}.
 
-  Notation STS := (leibnizO (STS_states * STS_rels)).
-  Notation STS_STD := (leibnizO (STS_std_states Addr region_type)).
-  Notation WORLD := (prodO STS_STD STS). 
-  Implicit Types W : WORLD.
-
-  Lemma registers_mapsto_resources pc_w stk_w rt0_w adv_w pc_w' (rmap: gmap RegName Word) :
-    dom (gset RegName) rmap = all_registers_s ∖ {[PC; r_stk; r_t0; r_t30]} →
-    ([∗ map] r_i↦_ ∈ rmap, r_i ↦ᵣ inl 0%Z)
-    -∗ r_stk ↦ᵣ stk_w
-    -∗ r_t0 ↦ᵣ rt0_w
-    -∗ r_t30 ↦ᵣ adv_w
-    -∗ PC ↦ᵣ pc_w'
-    -∗
-    registers_mapsto (<[PC:=pc_w']> (<[PC:=pc_w]> (<[r_stk:=stk_w]> (<[r_t0:=rt0_w]> (<[r_t30:=adv_w]>
-      (create_gmap_default (list_difference all_registers [PC; r_stk; r_t0; r_t30]) (inl 0%Z))))))).
-  Proof.
-    iIntros (Hdom) "Hregs Hr_stk Hr_t0 Hr_adv HPC".
-    rewrite /registers_mapsto insert_insert.
-    do 4 (rewrite big_sepM_insert; [iFrame|done]).
-    iDestruct (big_sepM_dom with "Hregs") as "Hregs".
-    iApply (big_sepM_mono (λ k _, k ↦ᵣ inl 0%Z))%I.
-    { intros * [? ->]%create_gmap_default_lookup_is_Some. auto. }
-    iApply big_sepM_dom. rewrite big_opS_proper'. iFrame. done.
-    rewrite Hdom.
-    rewrite create_gmap_default_dom list_to_set_difference -/all_registers_s.
-    f_equal. clear. set_solver.
-  Qed.
-
-  Lemma r_full (pc_w stk_w rt0_w adv_w : Word) :
-    full_map (Σ:=Σ) (<[PC:=pc_w]> (<[r_stk:=stk_w]> (<[r_t0:=rt0_w]> (<[r_t30:=adv_w]>
-           (create_gmap_default (list_difference all_registers [PC; r_stk; r_t0; r_t30]) (inl 0%Z)))))).
-  Proof.
-    rewrite /full_map. iPureIntro. intros rr. cbn beta.
-    rewrite elem_of_gmap_dom 4!dom_insert_L create_gmap_default_dom list_to_set_difference.
-    rewrite -/all_registers_s. generalize (all_registers_s_correct rr). clear. set_solver.
-  Qed.
+  (* -------------------------------- LTACS -------------------------------------- *)
   
+  (* Tactic for destructing a list into elements *)
+  Ltac destruct_list l :=
+    match goal with
+    | H : strings.length l = _ |- _ =>
+      let a := fresh "a" in
+      let l' := fresh "l" in
+      destruct l as [|a l']; [inversion H|];
+      repeat (let a' := fresh "a" in
+              destruct l' as [|a' l'];[by inversion H|]);
+      destruct l'; [|by inversion H]
+    end.
+
+  Ltac iPrologue_pre :=
+    match goal with
+    | Hlen : strings.length ?a = ?n |- _ =>
+      let a' := fresh "a" in
+      destruct a as [| a' a]; [inversion Hlen|]
+    end.
+
+  Ltac iPrologue prog :=
+    iDestruct prog as "[Hi Hprog]";
+    iApply (wp_bind (fill [SeqCtx])).
+
+  Ltac iEpilogue prog :=
+    iNext; iIntros prog; iSimpl;
+    iApply wp_pure_step_later;auto;iNext.
+
   Ltac middle_lt prev index :=
     match goal with
-    | Ha_first : ?a !! 0 = Some ?a_first |- _ 
+    | Ha_first : ?a !! 0 = Some ?a_first |- _
     => apply Z.lt_trans with prev; auto; apply incr_list_lt_succ with a index; auto
-    end. 
-
-  Ltac iContiguous_bounds i j :=
-    eapply contiguous_between_middle_bounds' with (a0 := i) (an := j);
-    [ eauto | cbn; solve [ repeat constructor ] ].
+    end.
 
   Ltac iCorrectPC i j :=
     eapply isCorrectPC_contiguous_range with (a0 := i) (an := j); eauto; [];
     cbn; solve [ repeat constructor ].
 
-  Ltac iContiguous_bounds_withinBounds a0 an :=
-    apply isWithinBounds_bounds_alt' with a0 an; auto; [];
-    iContiguous_bounds a0 an.
-
-  Lemma isCorrectPC_range_npE p g b e a0 an :
-    isCorrectPC_range p g b e a0 an →
-    (a0 < an)%a →
-    p ≠ E.
-  Proof.
-    intros HH1 HH2. 
-    destruct (isCorrectPC_range_perm _ _ _ _ _ _ HH1 HH2) as [?| [?|?] ]; 
-      congruence.
-  Qed.
-
-  Ltac isWithinBounds := rewrite /withinBounds; apply andb_true_iff; split; [apply Z.leb_le|apply Z.ltb_lt]; simpl; auto.
-
-  Ltac iNotElemOfList :=
-    repeat (apply not_elem_of_cons; split;[auto|]); apply not_elem_of_nil.  
-
-  Ltac addr_succ :=
-    match goal with
-    | H : _ |- (?a1 + ?z)%a = Some ?a2 =>
-      rewrite /incr_addr /=; do 2 f_equal; apply eq_proofs_unicity; decide equality
-    end.
-
-   (* The following ltac gets out the next general purpuse register *)
-   Ltac get_genpur_reg Hr_gen wsr ptr :=
-     let w := fresh "wr" in 
-       destruct wsr as [? | w wsr]; first (by iApply bi.False_elim);
-       iDestruct Hr_gen as ptr.
-
-   Ltac iDestructList Hlength l :=
-     (repeat (let a := fresh "a" in destruct l as [|a l];[by inversion Hlength|]));
-     destruct l;[|by inversion l].
-
-   Ltac iContiguous_next Ha index :=
+  Ltac iContiguous_next Ha index :=
     apply contiguous_of_contiguous_between in Ha;
     generalize (contiguous_spec _ Ha index); auto.
 
-   Ltac iPrologue_pre l Hl :=
-     destruct l; [inversion Hl|]; iApply (wp_bind (fill [SeqCtx])).
-   
-   Ltac iPrologue l Hl prog := 
-     iPrologue_pre l Hl;
-     iDestruct prog as "[Hinstr Hprog]".     
+  Ltac consider_next_reg r1 r2 :=
+    destruct (decide (r1 = r2));[subst;rewrite lookup_insert;eauto|rewrite lookup_insert_ne;auto]. 
 
-  Ltac iEpilogue intro_ptrn :=
-    iNext; iIntros intro_ptrn; iSimpl;
-    iApply wp_pure_step_later;auto;iNext.
+  (* ----------------------------------------------------------------------------- *)
+  Definition ro := encodePerm RO.
+  Definition roe_instrs f_m f_a r1 :=
+    malloc_instrs f_m 1%nat ++
+    [move_r r_env r_t1;
+    move_r r_t7 r_t1;
+    store_z r_env 1; 
+    restrict_z r_t7 ro] ++
+    call_instrs f_m (offset_to_cont_call [r_t7]) r1 [r_env] [r_t7] ++
+    restore_locals_instrs r_t2 [r_env] ++
+    [load_r r_t0 r_env] ++
+    assert_r_z_instrs f_a r_t0 1 ++
+    [halt].
 
-  Ltac iLookupR Hl :=
-    rewrite /= lookup_app_r;rewrite Hl /=;auto.
+  Definition roe a f_m f_a r1 :=
+    ([∗ list] a_i;w ∈ a;(roe_instrs f_m f_a r1), a_i ↦ₐ w)%I.
 
+  Definition roe_inv d : iProp Σ :=
+    (∃ w, d ↦ₐ w ∗ ⌜w = inl 1%Z⌝)%I.
 
-  (* encapsulation of local state using local capabilities and scall *)
-  (* assume r1 contains an executable pointer to adversarial code 
-     (no linking table yet) *)
-  Definition f2_instrs (r1 : RegName) epilogue_off f_a :=
-     [pushU_z_instr r_stk 1] ++
-     scallU_prologue_instrs epilogue_off r1 ++
-     [jmp r1;
-     sub_z_z r_t1 0 6;
-     lea_r r_stk r_t1] ++
-     popU_instrs r_stk r1 ++
-     assert_r_z_instrs f_a r1 1 ++
-     [halt].
+  Definition roeN : namespace := nroot .@ "roeN".
+  Definition roeN_link : namespace := roeN .@ "link".
+  Definition roeN_flag : namespace := roeN .@ "flag".
+  Definition roeN_act : namespace := roeN .@ "act".
+  Definition roeN_locals : namespace := roeN .@ "locals".
+  Definition roeN_b : namespace := roeN .@ "locals".
+  Definition roeN_prog : namespace := roeN .@ "prog".
 
-  Definition f2 (a : list Addr) (p : Perm) (r1 : RegName) flag_off : iProp Σ :=
-    ([∗ list] a_i;w_i ∈ a;(f2_instrs r1 40 flag_off), a_i ↦ₐ[p] w_i)%I.
-
-  (* Shorthand definition for an adress being currently temporary/revoked *)
-   Definition region_type_revoked W (a : Addr) :=
-     (std W) !! a = Some Revoked.
-   Definition region_type_temporary W (a : Addr) :=
-     (std W) !! a = Some Temporary.
-   Definition region_type_uninitialized W (a : Addr) :=
-     exists w, (std W) !! a = Some (Static {[a:=w]}).
-
-   Lemma region_type_temporary_dec W a: Decision (region_type_temporary W a).
-   Proof.
-     rewrite /region_type_temporary. solve_decision.
-   Qed.
-   
-   Lemma region_type_uninitialized_dec W a: Decision (region_type_uninitialized W a).
-   Proof.
-     rewrite /region_type_uninitialized. destruct (std W !! a); [|right; red; intros (w & A); discriminate].
-     destruct r; try (right; red; intros (w & A); discriminate).
-     destruct (g !! a) eqn:Hsome;[|right];[|intros [? ?];simplify_map_eq].
-     destruct (decide (g = {[a:=w]}));[left|right];subst;eauto. intros [? ?]. simplify_map_eq. 
-   Qed.
-
+  Definition r_adv := r_t31.
   
-  (* We want to show encapsulation of local state, by showing that an arbitrary adv 
-     cannot change what lies on top of the stack after return, i.e. we want to show
-     that the last pop indeed loads the value 1 into register r1 *)
-  (* to make the proof simpler, we are assuming WLOG the r1 registers is r_t30 *)
-  Lemma f2_spec W rmap pc_p pc_p' pc_g pc_b pc_e (* PC *)
-        f2_addrs (* f2 *)
-        f_b f_e f_a b_link e_link a_link a_entry (* linking table variables *)
-        f_a_first f_a_last flag_p flag_b flag_e flag_a a_env (* failure subroutine details *)
-        wadv (* adversary capability *)
-        a_first a_last (* special adresses *) 
-        (b_r e_r : Addr) (* stack *) :
-    
+  Lemma roe_spec pc_p pc_b pc_e (* PC *)
+        roe_addrs wadv (* program addresses *)
+        b_m e_m f_m mallocN (* malloc *)
+        b_link e_link a_link f_a a_entry a_entry' (* link *)
+        fail_start fail_end a_env (* fail *)
+        flag_p flag_b flag_e flag_a (* flag *)
+        a_first a_last (* special adresses *)
+        rmap (* registers *) :
+
     (* PC assumptions *)
-    isCorrectPC_range pc_p pc_g pc_b pc_e a_first a_last ->
-    PermFlows pc_p pc_p' ->
+    isCorrectPC_range pc_p pc_b pc_e a_first a_last ->
 
     (* Program adresses assumptions *)
-    contiguous_between f2_addrs a_first a_last ->
+    contiguous_between roe_addrs a_first a_last ->
 
-    (* Linking table and failure subroutine assumptions *)
-    withinBounds (RW, Global, b_link, e_link, a_entry) = true →
-    (a_link + f_a)%a = Some a_entry ->
-    (f_a_first + strings.length assert_fail_instrs)%a = Some a_env ->
-
-    (* We assume the adversary capability is Global *)
-    isLocalWord wadv = false ->
+    (* Assumptions about linking table *)
+    withinBounds (RW, b_link, e_link, a_entry) = true →
+    withinBounds (RW, b_link, e_link, a_entry') = true →
+    (a_link + f_m)%a = Some a_entry →
+    (a_link + f_a)%a = Some a_entry' →
+    (fail_start + strings.length (assert_fail_instrs))%a = Some a_env →
     
-    (* Stack assumptions *)
-    region_size b_r e_r > 8 -> (* we must assume the stack is large enough for needed local state *)
-
     (* footprint of the register map *)
-    dom (gset RegName) rmap = all_registers_s ∖ {[PC;r_stk;r_t30]} →
+    dom (gset RegName) rmap = all_registers_s ∖ {[PC;r_adv]} →
     
-    {{{ r_stk ↦ᵣ inr ((URWLX,Local),b_r,e_r,b_r)
-      ∗ interp W (inr ((URWLX,Local),b_r,e_r,b_r))
+    {{{ PC ↦ᵣ inr (pc_p,pc_b,pc_e,a_first)
+      ∗ r_adv ↦ᵣ wadv
       ∗ ([∗ map] r_i↦w_i ∈ rmap, r_i ↦ᵣ w_i)
-      (* flag *)
-      ∗ (∃ ι, inv ι (flag_a ↦ₐ[RW] inl 0%Z))
-      (* token which states all invariants are closed *)
+      (* token which states all non atomic invariants are closed *)
       ∗ na_own logrel_nais ⊤
-      (* adv *)
-      ∗ r_t30 ↦ᵣ wadv
-      ∗ interp W wadv
-      (* trusted *)
-      ∗ PC ↦ᵣ inr ((pc_p,pc_g),pc_b,pc_e,a_first)
-      ∗ f2 f2_addrs pc_p' r_t30 f_a
-      (* linking table *)
-      ∗ (pc_b ↦ₐ[pc_p'] inr (RO,Global,b_link,e_link,a_link)
-              ∗ a_entry ↦ₐ[RO] inr (E, Global, f_b, f_e, f_a_first))
-      (* failure subroutine *)
-      ∗ (∃ ι, na_inv logrel_nais ι (∃ a', ⌜contiguous_between a' f_a_first f_a_last⌝
-                                           ∗ assert_fail a' RX
-                                           ∗ a_env ↦ₐ[RX] inr (flag_p, Global, flag_b, flag_e, flag_a)))
-      (* we start out with arbitrary sts *)
-      ∗ sts_full_world W
-      ∗ region W
+      (* trusted code *)
+      ∗ roe roe_addrs f_m f_a r_adv
+      (* untrusted code *)
+      ∗ interp wadv
+      
+      (** Resources for malloc and assert **)
+      (* assume that a pointer to the linking table (where the malloc capa is) is at offset 0 of PC *)
+      ∗ na_inv logrel_nais mallocN (malloc_inv b_m e_m)
+      ∗ pc_b ↦ₐ (inr (RO, b_link, e_link, a_link))
+      ∗ a_entry ↦ₐ (inr (E, b_m, e_m, b_m))
+      ∗ a_entry' ↦ₐ (inr (E, fail_start, fail_end, fail_start))
+      ∗ a_env ↦ₐ inr (flag_p, flag_b, flag_e, flag_a)
+      (* invariant about the failure flag *)
+      ∗ (inv roeN_flag (flag_a ↦ₐ inl 0%Z))
     }}}
       Seq (Instr Executable)
-    {{{ v, RET v; ⌜v = HaltedV⌝ →
-                    ∃ r W', full_map r ∧ registers_mapsto r
-                         ∗ ⌜related_sts_priv_world W W'⌝
-                         ∗ na_own logrel_nais ⊤                           
-                         ∗ sts_full_world W'
-                         ∗ region W' }}}.
+      {{{ v, RET v; True }}}. (* in this spec, we do not care about the postcondition, 
+                              only that the flag invariant holds throughout the program, 
+                              and that the program does not get stuck *)
   Proof.
-    iIntros (Hvpc Hfl Hf2 Hwb_link Ha_entry Ha_env Hglobal Hsize Hrmap_dom φ)
-            "(Hr_stk & #Hstk_val & Hr_gen & #Hflag & Hna & Hr_adv & #Hadv & HPC & Hf2 & Hlink & #Hfail & Hs & Hr) Hφ /=".
-    (* prepare stack validity *)
-    rewrite fixpoint_interp1_eq. iSimpl in "Hstk_val".
-    assert (min b_r e_r = b_r) as ->.
-    { revert Hsize; rewrite /region_size;clear. solve_addr. }
-    assert (region_addrs b_r b_r = []) as ->;[by rewrite /region_addrs /region_size -Zminus_diag_reverse /=|].
-    assert (max b_r b_r = b_r) as ->;[clear;solve_addr|].
-    iDestruct "Hstk_val" as "[_ Hstk_val]".
-    iAssert ([∗ list] a' ∈ region_addrs b_r e_r, read_write_cond a' RWLX (fixpoint interp1) ∧ ⌜region_state_U_pwl W a'⌝)%I
-      as "#Hstk_region".
-    { iApply (big_sepL_mono with "Hstk_val"). iIntros (k y Hy) "H".
-      iDestruct "H" as (p Hfl') "H". destruct p;inversion Hfl'. iFrame. }
+    iIntros (Hvpc Hcont Hwb1 Hwb2 Ha_entry Ha_entry' Ha_env Hdom φ) 
+            "(HPC & Hr_adv & Hregs & Hown & Hprog & #Hwadv & #Hmalloc & Hpc_b & Ha_entry & Ha_entry' & Ha_env & #Hflag) Hφ". 
+    (* extract r_t0 *)
+    assert (is_Some (rmap !! r_t0)) as [w0 Hw0].
+    { apply elem_of_gmap_dom. rewrite Hdom. clear;set_solver. }
+    iDestruct (big_sepM_delete with "Hregs") as "[Hr_t0 Hregs]";[apply Hw0|]. 
+    (* put back r_adv *)
+    iDestruct (big_sepM_insert with "[$Hregs $Hr_adv]") as "Hregs". 
+    { rewrite lookup_delete_ne;auto. apply elem_of_gmap_dom_none. rewrite Hdom. clear;set_solver. }
 
-    (* next we will need to split the stack into its temporary and uninitialized parts, revoke it, and manually revoke 
-       the uninitialised parts of the desired local stack frame *)
-    destruct (region_addrs_split3 _ _ _ Hsize) as [asplit [Hstksplit Hspliteq] ].
-    set (ltempsplit := (@list_filter Addr (region_type_temporary W) (region_type_temporary_dec W)
-                                     (region_addrs b_r asplit))).
-    set (ltemp := (@list_filter Addr (region_type_temporary W) (region_type_temporary_dec W)
-                                (region_addrs b_r e_r))).
-    set (ltemprest := (@list_filter Addr (region_type_temporary W) (region_type_temporary_dec W)
-                                    (region_addrs asplit e_r))).
-    assert (Hltempspliteq: ltemp = ltempsplit ++ ltemprest).
-    { rewrite /ltemp /ltempsplit /ltemprest.
-      rewrite Hstksplit list_filter_app. auto. }
-    iAssert (⌜Forall (λ a, region_type_temporary W a) ltemp⌝)%I as %Htemp.
-    { iPureIntro. eapply List.Forall_forall.
-      intros. eapply elem_of_list_filter.
-      eapply elem_of_list_In; eauto. }
-    remember Htemp as Htemp'. clear HeqHtemp'.
-    rewrite Hltempspliteq in Htemp. eapply Forall_app in Htemp.
-    destruct Htemp as [Htemp Htemprest].
-    set (luninitsplit := (@list_filter Addr (region_type_uninitialized W) (region_type_uninitialized_dec W)
-                                       (region_addrs b_r asplit))).
-    iAssert (⌜Forall (λ a, region_type_uninitialized W a) luninitsplit⌝)%I as %Huninit.
-    { iPureIntro. eapply List.Forall_forall.
-      intros. eapply elem_of_list_filter.
-      eapply elem_of_list_In; eauto. }
-    assert (Hdupuninit: NoDup luninitsplit).
-    { eapply NoDup_filter, NoDup_ListNoDup. apply NoDup_ListNoDup,region_addrs_NoDup. }
-    pose proof (extract_temps_split W ltemp) as [l' [Hdup Hiff] ];
-      [apply NoDup_filter,NoDup_ListNoDup,NoDup_ListNoDup, region_addrs_NoDup|apply Htemp'|].
+    (* prepare the program addresses for malloc *)
+    iDestruct (contiguous_between_program_split with "Hprog") as
+        (ai_malloc ai_rest a_malloc_end) "(Hmalloc_prog & Hprog & #Hcont)"; [apply Hcont|].
+    iDestruct "Hcont" as %(Hcont_malloc & Hcont_rest & Heqapp & Hlink).
+    iDestruct (big_sepL2_length with "Hmalloc_prog") as %Hai_malloc_len.
+    assert (isCorrectPC_range pc_p pc_b pc_e a_first a_malloc_end) as Hvpc1.
+    { eapply isCorrectPC_range_restrict. apply Hvpc.
+      generalize (contiguous_between_bounds _ _ _ Hcont_rest). clear; solve_addr. }
+    assert (isCorrectPC_range pc_p pc_b pc_e a_malloc_end a_last) as Hvpc2.
+    { eapply isCorrectPC_range_restrict. apply Hvpc.
+      generalize (contiguous_between_bounds _ _ _ Hcont_malloc). clear; solve_addr. }
+    rewrite -/(malloc _ _ _ _).
+    (* apply the malloc spec *)
+    iApply (malloc_spec_alt with "[- $Hφ $HPC $Hmalloc_prog $Hpc_b $Ha_entry $Hr_t0 $Hregs $Hmalloc $Hown]");
+      [apply Hvpc1|eapply Hcont_malloc|eapply Hwb1|eapply Ha_entry| |auto|lia|..].
+    { rewrite !dom_insert_L !dom_delete_L Hdom !difference_difference_L. clear. set_solver. }
+    iSplitR;[iNext;auto|]. 
+    iNext. iIntros "(HPC & Hmalloc_prog & Hpc_b & Ha_entry & Hbe & Hr_t0 & Hown & Hregs)".
+    iDestruct "Hbe" as (b e Hincr) "(Hr_t1 & Hbe)". 
+    iDestruct (region_mapsto_single with "Hbe") as (cellv) "(Hbe & _)". revert Hincr; clear; solve_addr.
 
-    (* we revoke all temporary regions in W *)
-    iMod (monotone_revoke_keep_some W _ ltemp with "[$Hs $Hr]") as "[Hsts [Hr [Hrest Hstack] ] ]";[apply Hdup|..].
-    { iSplit.
-      - iApply big_sepL_forall. iPureIntro. intros n. simpl. intros x Hsome. apply Hiff. apply elem_of_app; left.
-        apply elem_of_list_lookup. eauto. 
-      - iApply big_sepL_forall. iIntros. iSplit.
-        + iPureIntro. eapply Hiff, elem_of_app; right.
-          eapply elem_of_list_lookup; eauto.
-        + generalize (proj2 (elem_of_list_lookup ltemp x) ltac:(eauto)); intro Hx.
-          eapply elem_of_list_filter in Hx. destruct Hx as [Hx1 Hx2].
-          iDestruct (big_sepL_elem_of with "Hstk_region") as "[H _]"; eauto.
-          rewrite /read_write_cond /=. iApply "H". }
-    rewrite Hltempspliteq. iDestruct (big_sepL_app with "Hstack") as "[Hstack Hstackrest]".
+    (* extract r_env and r_t7 *)
+    assert (is_Some (rmap !! r_env)) as [wenv Hwenv].
+    { apply elem_of_gmap_dom. rewrite Hdom. clear;set_solver. }
+    iDestruct (big_sepM_delete _ _ r_env with "Hregs") as "[Hr_env Hregs]";[rewrite !lookup_insert_ne// lookup_delete_ne//
+                                                                                    !lookup_insert_ne// lookup_delete_ne//|].
+    assert (is_Some (rmap !! r_t7)) as [w7 Hw7].
+    { apply elem_of_gmap_dom. rewrite Hdom. clear;set_solver. }
+    iDestruct (big_sepM_delete _ _ r_t7 with "Hregs") as "[Hr_t7 Hregs]";[rewrite lookup_delete_ne// !lookup_insert_ne// lookup_delete_ne//
+                                                                                    !lookup_insert_ne// lookup_delete_ne//|].
+    (* continue *)
+    iDestruct (big_sepL2_length with "Hprog") as %Hlength_rest.
+    destruct ai_rest as [|? ai_rest];[inversion Hlength_rest|].
+    apply contiguous_between_cons_inv_first in Hcont_rest as Heq; subst a. 
+    (* move r_env r_t1 *)
+    destruct ai_rest as [|? ai_rest];[inversion Hlength_rest|].
+    iPrologue "Hprog".
+    iApply (wp_move_success_reg with "[$HPC $Hi $Hr_env $Hr_t1]");
+      [apply decode_encode_instrW_inv|iCorrectPC a_malloc_end a_last|iContiguous_next Hcont_rest 0|]. 
+    iEpilogue "(HPC & Hi & Hr_env & Hr_t1)". iCombine "Hi" "Hmalloc_prog" as "Hprog_done".
+    (* move r_t7 r_t1 *)
+    destruct ai_rest as [|? ai_rest];[inversion Hlength_rest|].
+    iPrologue "Hprog".
+    iApply (wp_move_success_reg with "[$HPC $Hi $Hr_t7 $Hr_t1]");
+      [apply decode_encode_instrW_inv|iCorrectPC a_malloc_end a_last|iContiguous_next Hcont_rest 1|]. 
+    iEpilogue "(HPC & Hi & Hr_t7 & Hr_t1)". iCombine "Hi" "Hprog_done" as "Hprog_done". 
+    (* store r_env 1 *)
+    destruct ai_rest as [|? ai_rest];[inversion Hlength_rest|].
+    iPrologue "Hprog".
+    iApply (wp_store_success_z with "[$HPC $Hi $Hr_env $Hbe]");
+      [apply decode_encode_instrW_inv|iCorrectPC a_malloc_end a_last|iContiguous_next Hcont_rest 2|..].
+    { split;auto. rewrite andb_true_iff Z.leb_le Z.ltb_lt. clear -Hincr. solve_addr. }
+    iEpilogue "(HPC & Hi & Hr_env & Hbe)". iCombine "Hi" "Hprog_done" as "Hprog_done". 
+    (* restrict r_t7 RO *)
+    destruct ai_rest as [|? ai_rest];[inversion Hlength_rest|].
+    iPrologue "Hprog".
+    iApply (wp_restrict_success_z with "[$HPC $Hi $Hr_t7]");
+      [apply decode_encode_instrW_inv|iCorrectPC a_malloc_end a_last|iContiguous_next Hcont_rest 3|auto..].
+    { rewrite decode_encode_perm_inv. auto. }
+    iEpilogue "(HPC & Hi & Hr_t7)". iCombine "Hi" "Hprog_done" as "Hprog_done". 
 
-    (* Revoke some uninitialized to get their points to *)
-    iMod (region_uninitialized_to_revoked W _ _ _ Hdupuninit with "[$Hsts $Hr]") as "HHH".
-    { iApply big_sepL_forall. iIntros. iSplit.
-      - iPureIntro. eapply (proj1 (elem_of_list_filter (region_type_uninitialized W) _ _)).
-        eapply elem_of_list_lookup. exists k. eauto.
-      - generalize (proj2 (elem_of_list_lookup luninitsplit x) ltac:(eauto)); intro Hx.
-        eapply elem_of_list_filter in Hx. destruct Hx as [Hx1 Hx2].
-        eapply elem_of_submseteq in Hx2;
-          [|eapply (submseteq_inserts_r (region_addrs asplit e_r) (region_addrs b_r asplit) (region_addrs b_r asplit));
-            auto].
-        rewrite -Hstksplit in Hx2.
-        iDestruct (big_sepL_elem_of with "Hstk_region") as "[H _]"; eauto.
-        rewrite /read_write_cond /=. iApply "H". }
+    (* prepare the program addresses for call *)
+    iDestruct (contiguous_between_program_split with "Hprog") as
+        (ai_call ai_rest' a_call_end) "(Hcall_prog & Hprog & #Hcont)".
+    { repeat (apply contiguous_between_cons_inv in Hcont_rest as [_ [? [_ Hcont_rest] ] ];
+        apply contiguous_between_cons_inv_first in Hcont_rest as Heq'; subst x). apply Hcont_rest. }
+    iDestruct "Hcont" as %(Hcont_call & Hcont_rest' & Heqapp' & Hlink').
+    iDestruct (big_sepL2_length with "Hcall_prog") as %Hai_call_len.
+    assert (isCorrectPC_range pc_p pc_b pc_e a2 a_call_end) as Hvpc3.
+    { eapply isCorrectPC_range_restrict. apply Hvpc.
+      generalize (contiguous_between_bounds _ _ _ Hcont_rest').
+      generalize (contiguous_between_bounds _ _ _ Hcont_malloc).
+      apply contiguous_between_middle_bounds' with (ai:=a2) in Hcont_rest;[|repeat constructor].
+      clear -Hcont_rest; solve_addr. }
+    assert (isCorrectPC_range pc_p pc_b pc_e a_call_end a_last) as Hvpc4.
+    { eapply isCorrectPC_range_restrict. apply Hvpc.
+      generalize (contiguous_between_bounds _ _ _ Hcont_call).
+      generalize (contiguous_between_bounds _ _ _ Hcont_malloc).
+      apply contiguous_between_middle_bounds' with (ai:=a2) in Hcont_rest;[|repeat constructor]. 
+      clear -Hcont_rest; solve_addr. }
+    (* prepare the registers *)
+    iDestruct (big_sepM_delete _ _ r_adv with "Hregs") as "[Hr_adv Hregs]";[rewrite !lookup_delete_ne// !lookup_insert_ne//
+                                                                                    lookup_delete_ne//; apply lookup_insert|].
+    rewrite (delete_insert_ne _ _ r_adv)// !(insert_commute _ _ r_adv)// (delete_insert_ne _ _ r_adv)// (delete_insert_ne _ _ r_adv)// delete_insert.
+    2: { rewrite !lookup_delete_ne// !lookup_insert_ne// !lookup_delete_ne//. apply elem_of_gmap_dom_none. rewrite Hdom. clear; set_solver. }
+    iDestruct (big_sepM_insert with "[$Hregs $Hr_t1]") as "Hregs";[rewrite !lookup_delete_ne// !lookup_insert_ne//; apply lookup_delete|].
+    rewrite -!(delete_insert_ne _ r_t1)// 2!(delete_commute _ _ r_t1)// insert_delete. 
+    (* apply the call spec *)
+    iApply (wp_wand _ _ _ (λ v0 : language.val cap_lang, True ∨ ⌜v0 = FailedV⌝)%I with "[-]");[|auto].
+    rewrite -/(call _ _ _ _). 
+    iApply (call_spec r_adv {[r_env:=inr (RWX, b, e, b)]} {[r_t7:=inr (decodePerm ro, b, e, b)]} _
+                      _ (delete r_t7 (delete r_t0 rmap))
+              with "[- $HPC $Hown $Hmalloc $Hpc_b $Ha_entry $Hr_adv $Hregs]");
+      [apply Hvpc3|apply Hcont_call|auto|apply Ha_entry|..|solve_ndisj|]. 
+    { rewrite map_to_list_singleton. auto. }
+    { rewrite !dom_singleton_L dom_insert_L !dom_delete_L !dom_insert_L !dom_delete_L Hdom. clear.
+      rewrite !union_assoc_L !difference_difference_L !union_assoc_L union_comm_L (union_comm_L {[r_t2; r_t3; r_t4; r_t5]}).
+      rewrite difference_union_distr_l_L. set_solver. }
+    { rewrite dom_singleton_L !dom_delete_L Hdom. clear. set_solver. }
+    { rewrite !dom_insert_L !dom_delete_L !dom_insert_L dom_delete_L !union_assoc_L Hdom !difference_difference_L. clear. 
+      rewrite -!(union_assoc_L {[r_t1]}). apply union_mono_l. apply subseteq_difference_r;[set_solver|].
+      apply union_mono_l. apply subseteq_difference_r;[set_solver|]. apply all_registers_subseteq. }
+    rewrite !map_to_list_singleton. iSimpl. rewrite /call. iFrame "Hcall_prog". 
+    iSplitL "Hr_t7". iNext. iApply big_sepM_singleton. iFrame.  
+    iSplitL "Hr_t0". iNext. eauto.
+    iSplitL "Hr_env". iNext. iApply big_sepM_singleton. iFrame.
+    (* in anticipation of the result of the call macro, we create the callback now *)
+    iDestruct (jmp_or_fail_spec with "Hwadv") as "Hcallback_now".
+    destruct (decide (isCorrectPC (updatePcPerm wadv))).
+    2: { iNext. iIntros "Hbc". iDestruct "Hbc" as (b_c e_c b_l e_l a_end Hnext) "(HPC & _)". iApply "Hcallback_now". iFrame. }
+    iDestruct "Hcallback_now" as (p b' e' a' ->) "Hcallback_now". 
+    (* continue the program, now pointing at the adversary *)
+    iNext. iIntros "Hbc".
+    iDestruct "Hbc" as (b_c e_c b_l e_l a_end Hnext) "(HPC & Hregs & Hr_t7 & Hpc_b & Ha_entry & Hr_adv & Hr_t0 & Hbec & Hbel & Hcall_prog & Hown)".
+    (* cleanup *)
+    iDestruct (big_sepM_singleton (λ k i, k ↦ᵣ i)%I with "Hr_t7") as "Hr_t7".
+    iCombine "Hcall_prog" "Hprog_done" as "Hprog_done". 
+
+    (* we are now ready to call the unknown adversary *)
+    (* we first need to prepare the invariants needed *)
+    iMod (na_inv_alloc logrel_nais _ roeN_act with "Hbec") as "#Hbec". 
+    iMod (na_inv_alloc logrel_nais _ roeN_locals with "Hbel") as "#Hbel".
+    iCombine "Ha_entry' Ha_env Hpc_b Ha_entry" as "Hlink". 
+    iMod (na_inv_alloc logrel_nais _ roeN_link with "Hlink") as "#Hlink". 
+    iMod (inv_alloc (logN.@b) _ (roe_inv b) with "[Hbe]") as "#Hb". 
+    { iNext. iExists _; iFrame. auto. }
+    iMod (na_inv_alloc logrel_nais _ roeN_prog with "Hprog") as "#Hprog".
+    iClear "Hprog_done".
     
-    iDestruct "HHH" as "[Hsts [Hr Huninitstack]]".
+    (* Let's assert that the continuation holds *)
+    iDestruct (big_sepM_to_create_gmap_default _ _ (λ k i, k ↦ᵣ i)%I (inl 0%Z) with "Hregs")  as "Hregs";[apply Permutation_refl|reflexivity|]. 
+    iDestruct (big_sepM_insert with "[$Hregs $Hr_adv]") as "Hregs".
+    { apply elem_of_gmap_dom_none. rewrite create_gmap_default_dom list_to_set_map_to_list !dom_delete_L Hdom. clear. set_solver. }
+    iDestruct (big_sepM_insert with "[$Hregs $Hr_t7]") as "Hregs".
+    { apply elem_of_gmap_dom_none. rewrite !dom_insert_L create_gmap_default_dom list_to_set_map_to_list !dom_delete_L Hdom. clear. set_solver. }
+    iDestruct (big_sepM_insert with "[$Hregs $Hr_t0]") as "Hregs".
+    { apply elem_of_gmap_dom_none. rewrite !dom_insert_L create_gmap_default_dom list_to_set_map_to_list !dom_delete_L Hdom. clear. set_solver. }
+    iDestruct (big_sepM_insert with "[$Hregs $HPC]") as "Hregs".
+    { apply elem_of_gmap_dom_none. rewrite !dom_insert_L create_gmap_default_dom list_to_set_map_to_list !dom_delete_L Hdom. clear. set_solver. }
     
-    set (W' := (std_update_multiple (revoke W) luninitsplit Revoked)).
-    iAssert ((▷ ∃ ws, ([∗ list] a;w ∈ region_addrs b_r asplit;ws, a ↦ₐ[RWLX] w))
-               ∗ ⌜Forall (λ a : Addr, region_type_revoked W' a) ltempsplit⌝
-               ∗ ⌜Forall (λ a : Addr, region_type_revoked W' a) luninitsplit⌝)%I
-      with "[Hstack Huninitstack]" as "[>Hstack [#Hrevoked1 #Hrevoked2]]".
-    { iDestruct (big_sepL_sep with "Hstack") as "[Hstack #Hrevoked]".
-      iDestruct (big_sepL_forall with "Hrevoked") as %Hrevoked.
-      rename Hrevoked into Hrevoked'.
-      assert (Hrevoked: ∀ (x : nat) (x0 : Addr), ltempsplit !! x = Some x0 → std (revoke W) !! x0 = Some Revoked).
-      { intros. eapply Hrevoked'. rewrite Hltempspliteq. eauto. }
-      iSplit;[|iPureIntro].
-      - iDestruct (big_sepL_sep with "Hstack") as "[Hstack _]". iNext.
-        iApply region_addrs_exists.
-        iDestruct (region_addrs_exists with "Hstack") as (ws) "Hstack".
-        iDestruct (big_sepL2_sep with "Hstack") as "[_ Hstack]".
-        iDestruct (big_sepL2_sep with "Hstack") as "[Hstack _]".
-        iDestruct (region_addrs_exists with "[Hstack]") as "Hstack".
-        { iExists ws; auto. }
-        iAssert (∀ x : Addr, ⌜x ∈ region_addrs b_r asplit⌝ →
-                             ⌜region_type_temporary W x ∨ region_type_uninitialized W x⌝)%I as %HHH.
-        { iIntros. eapply elem_of_submseteq in a; [|eapply (submseteq_inserts_r (region_addrs asplit e_r)
-                                                                                (region_addrs b_r asplit)
-                                                                                (region_addrs b_r asplit)); auto].
-          rewrite -Hstksplit in a.
-          iDestruct (big_sepL_elem_of with "Hstk_region") as "[_ %]"; eauto. }
-        iApply (big_sepL_merge with "[$Hstack] [$Huninitstack]").
-        { eapply NoDup_ListNoDup,NoDup_ListNoDup,region_addrs_NoDup. }
-        { intros. destruct (HHH _ H) as [HH|HH].
-          - left. eapply elem_of_list_filter; auto.
-          - right. eapply elem_of_list_filter; auto. }
-      - split.
-        + revert Htemp; repeat (rewrite Forall_forall). 
-          intros Htemp x Hx. eapply elem_of_list_lookup in Hx.
-          destruct Hx. rewrite /W' /region_type_revoked std_sta_update_multiple_lookup_same_i.
-          eapply Hrevoked; eauto.
-          red; intro. eapply elem_of_list_filter in H0. destruct H0.
-          eapply Hrevoked in H. destruct H0.
-          rewrite /revoke /revoke_std_sta lookup_fmap H0 /= in H.
-          discriminate.
-        + eapply Forall_forall. intros. rewrite /W' /region_type_revoked.
-          eapply std_sta_update_multiple_lookup_in_i; auto. }
-    iDestruct "Hrevoked1" as %Hrevoked1.
-    iDestruct "Hrevoked2" as %Hrevoked2.
-    (* we prepare the stack for storing local state *)
-    (* Splitting the stack into own and adv parts *)
-    assert (contiguous (region_addrs b_r e_r)) as Hcont_stack;[apply region_addrs_contiguous|].
-    assert (contiguous_between (region_addrs b_r e_r) b_r e_r) as Hcontiguous.
-    { apply contiguous_between_of_region_addrs; auto. revert Hsize. rewrite /region_size. clear. solve_addr. }
-    iDestruct "Hstack" as (ws) "Hstack".
-    iDestruct (big_sepL2_length with "Hstack") as %Hlength.
-    assert (∃ ws_own ws_adv, ws = ws_own ++ ws_adv ∧ length ws_own = 8)
-      as [ws_own [ws_adv [Happ Hlength'] ] ].
-    { exists ws, []. split; auto. rewrite app_nil_r. auto.
-      rewrite -Hlength. rewrite region_addrs_length; auto. }
-    rewrite Happ. assert (Hcontiguous': contiguous_between (region_addrs b_r asplit) b_r asplit).
-    { eapply contiguous_between_of_region_addrs; auto.
-      rewrite /region_size in Hspliteq. revert Hspliteq; clear; solve_addr. }
-    iDestruct (contiguous_between_program_split with "Hstack") as
-        (stack_own stack_adv stack_own_last) "(Hstack_own & Hstack_adv & #Hcont)"; [eauto|].
-    iDestruct "Hcont" as %(Hcont1 & Hcont2 & Hstack_eq1 & Hlink1).
-    iDestruct (big_sepL2_length with "Hstack_own") as %Hlength_own. rewrite Hlength' in Hlength_own.
-    rewrite Hstack_eq1 in Hcontiguous'.
-    (* The following length assumptions will let us destruct the stack/program *)
-    iDestruct (big_sepL2_length with "Hf2") as %Hlength_f2.
-    iDestruct (big_sepL2_length with "Hstack_adv") as %Hlength_adv.
-    (* Getting the top adress on the stack *)
-    do 2 (destruct stack_own; [inversion Hlength_own|]; destruct ws_own;[inversion Hlength'|]).
-    assert ((region_addrs b_r asplit) !! 0 = Some b_r) as Hfirst_stack.
-    { apply region_addrs_first. revert Hspliteq; clear. rewrite /region_size. solve_addr. }
-    rewrite Hstack_eq1 /= in Hfirst_stack. inversion Hfirst_stack as [Heq]. subst b_r.
-    (* assert that the stack bounds are within bounds *)
-    assert (withinBounds (RWLX,Local,a,e_r,a) = true
-            ∧ withinBounds (RWLX,Local,a,e_r,stack_own_last) = true) as [Hwb1 Hwb2].
-    { split; isWithinBounds; first lia.
-      - revert Hsize. rewrite /region_size. clear. solve_addr.
-      - by eapply contiguous_between_bounds.
-      - apply contiguous_between_bounds in Hcont2. simplify_eq.
-        revert Hlength' Hlength Hlink1 Hsize Hlength_adv Hlength_own Hcont2.
-        rewrite -region_addrs_length app_length. clear.
-        rewrite !region_addrs_length /region_size. solve_addr.
-    }
-    (* push r_stk 1 *)
-    iDestruct "Hstack_own" as "[Ha Hstack_own]".
-    do 2 (destruct f2_addrs;[inversion Hlength_f2|]).
-    apply contiguous_between_cons_inv_first in Hf2 as Heq. subst a1. 
-    iDestruct (big_sepL2_app_inv _ [a_first] (a2::f2_addrs) with "Hf2") as "[Hpush Hprog]"; [simpl;auto|].
-    iDestruct "Hpush" as "[Hpush _]".
-    iApply (pushU_z_spec); [..|iFrame "HPC Hr_stk Ha Hpush"];
-      [iCorrectPC a_first a_last|apply Hfl|auto|iContiguous_next Hf2 0|iContiguous_next Hf2 0|auto|..].
-    { done. }
-    { iContiguous_next Hcont1 0. }
-    iNext. iIntros "(HPC & Hpush & Hr_stk & Hb_r)".
-    (* Prepare the scall prologue macro *)
-    rename a0 into stack_own_b.
-    (* destruct stack_own as [|stack_own_b stack_own];[inversion Hlength_own|]. *)
-    assert ((stack_own_b :: stack_own) = region_addrs stack_own_b stack_own_last) as ->.
-    { apply region_addrs_of_contiguous_between; auto.
-      repeat (inversion Hcont1 as [|????? Hcont1']; subst; auto; clear Hcont1; rename Hcont1' into Hcont1). }
-    (* assert (stack_adv = region_addrs stack_own_last e_r) as ->. *)
-    (* { apply region_addrs_of_contiguous_between; auto. } *)
-    assert (contiguous_between (a2 :: f2_addrs) a2 a_last) as Hcont_weak.
-    { repeat (inversion Hf2 as [|????? Hf2']; subst; auto; clear Hf2; rename Hf2' into Hf2). }
-    iDestruct (contiguous_between_program_split with "Hprog") as (scall_prologue rest s_last)
-                                                                   "(Hscall & Hf2 & #Hcont)"; [eauto|..].
-    clear Hfirst_stack Hcont_weak.
-    iDestruct "Hcont" as %(Hcont_scall & Hcont_rest & Hrest_app & Hlink).
-    iDestruct (big_sepL2_length with "Hscall") as %Hscall_length. simpl in Hscall_length, Hlength_f2.
-    assert ((stack_own_b + 7)%a = Some stack_own_last) as Hstack_own_bound.
-    { rewrite -(addr_add_assoc a _ 1). assert ((1 + 7) = 8)%Z as ->;[done|].
-      rewrite Hlength_own in Hlink1. revert Hlink1; clear; solve_addr.
-      apply contiguous_between_incr_addr with (i:=1) (ai:=stack_own_b) in Hcont1; auto. }
-    assert (∃ a, (stack_own_b + 6)%a = Some a) as [stack_own_end Hstack_own_bound'].
-    { revert Hstack_own_bound. clear. intros H. destruct (stack_own_b + 6)%a eqn:Hnone; eauto. solve_addr. }
-    assert (a2 < s_last)%a as Hcontlt.
-    { revert Hscall_length Hlink. clear. solve_addr. }
-    assert (a_first <= a2)%a as Hcontge.
-    { apply region_addrs_of_contiguous_between in Hcont_scall. simplify_eq.
-      revert Hscall_length Hf2 Hcontlt. clear =>Hscall_length Hf2 Hcontlt.
-      apply contiguous_between_middle_bounds with (i := 1) (ai := a2) in Hf2;[solve_addr|auto]. 
-    }
-    (* apply the uscall spec *)
-    iApply (scallU_prologue_spec with "[- $HPC $Hr_stk $Hscall $Hstack_own $Hr_gen]");
-      [ | |apply Hwb2| |apply Hcont_scall|apply Hfl|iNotElemOfList|
-        iContiguous_next Hcont1 2|apply Hstack_own_bound'|apply Hstack_own_bound| |done|..].
-    { assert (s_last <= a_last)%a as Hle;[by apply contiguous_between_bounds in Hcont_rest|].
-      intros mid Hmid. apply isCorrectPC_inrange with a_first a_last; auto.
-      revert Hle Hcontlt Hcontge Hmid. clear. intros. split; solve_addr. }
-    { simplify_eq. iContiguous_bounds_withinBounds a stack_own_last. }
-    { clear; split; solve_addr. }
-    { assert (5 + 40 = 45)%Z as ->;[done|]. rewrite Hscall_length in Hlink. done. }
-    iNext. iIntros "(HPC & Hr_stk & Hr_t0 & Hr_gen & Hstack_own & Hscall)".
-    iDestruct (big_sepL2_length with "Hf2") as %Hf2_length. simpl in Hf2_length.
-    assert (isCorrectPC_range pc_p pc_g pc_b pc_e s_last a_last) as Hvpc1.
-    { intros mid Hmid. assert (a_first <= s_last)%a as Hle;[apply contiguous_between_bounds in Hcont_scall;
-                                                           revert Hcont_scall Hcontge;clear; solve_addr|].
-      apply isCorrectPC_inrange with a_first a_last; auto.
-      revert Hmid Hle. clear. solve_addr. }
+    match goal with |- context [ ([∗ map] k↦y ∈ ?regs, k ↦ᵣ y)%I ] =>
+          set rmap2 := regs
+    end.
+    iSpecialize ("Hcallback_now" $! rmap2). rewrite /interp_expr. 
+    iDestruct ("Hcallback_now" with "[Hregs $Hown]") as "[_ Hconf]". 
+    { rewrite /registers_mapsto /rmap2. rewrite insert_insert. iFrame. 
+      iSplit.
+      { iPureIntro. intros x. simpl.
+        consider_next_reg x PC. consider_next_reg x r_t0. consider_next_reg x r_t7. consider_next_reg x r_adv.
+        apply elem_of_gmap_dom. rewrite create_gmap_default_dom list_to_set_map_to_list !dom_delete_L Hdom. clear -n n0 n1 n2.
+        repeat (apply elem_of_difference; split; [|set_solver]). apply all_registers_s_correct. }
+      iIntros (r Hne). 
+      rewrite /RegLocate. rewrite lookup_insert_ne;auto. 
+      consider_next_reg r r_t0;[|consider_next_reg r r_t7;[|consider_next_reg r r_adv] ].
+      - (* continuation *) iClear "Hcallback_now Hwadv".
+        rewrite !fixpoint_interp1_eq.
+        iIntros (r). iNext. iAlways.
+        iIntros "([% #Hreg_val] & Hreg & Hown)". iSplit;auto.
+        rewrite /interp_conf.
+        (* get the registers we need *)
+        iDestruct (big_sepM_delete _ _ PC with "Hreg") as "[HPC Hreg]"; [rewrite lookup_insert;eauto|].
+        rewrite delete_insert_delete.
+        assert (is_Some (r !! r_t1)) as [wrt1 Hwrt1];[auto|].
+        iDestruct (big_sepM_delete _ _ r_t1 with "Hreg") as "[Hr_t1 Hreg]"; [rewrite lookup_delete_ne//;eauto|].
+        assert (is_Some (r !! r_t2)) as [wrt2 Hwrt2];[auto|].
+        iDestruct (big_sepM_delete _ _ r_t2 with "Hreg") as "[Hr_t2 Hreg]"; [rewrite !lookup_delete_ne//;eauto|].
+        assert (is_Some (r !! r_env)) as [wenv' Hwenv'];[auto|].
+        iDestruct (big_sepM_delete _ _ r_env with "Hreg") as "[Hr_env Hreg]"; [rewrite !lookup_delete_ne//;eauto|].
+        assert (is_Some (r !! r_t0)) as [wrt0 Hwrt0];[auto|].
+        iDestruct (big_sepM_delete _ _ r_t0 with "Hreg") as "[Hr_t0 Hreg]"; [rewrite !lookup_delete_ne//;eauto|].
+        assert (is_Some (r !! r_t3)) as [wrt3 Hwrt3];[auto|].
+        iDestruct (big_sepM_delete _ _ r_t3 with "Hreg") as "[Hr_t3 Hreg]"; [rewrite !lookup_delete_ne//;eauto|].
 
-    (* We are now ready to set up the region invariants that we will use for the adversary call *)
-    (* Since we will halt once they return, we do not mind being in a private future world *)
-    (* We can therefore go the simple way and create a custom invariant for the local stack frame *)
+        (* step through the activation record *)
+        iMod (na_inv_open with "Hprog Hown") as "[>Hprog' [Hown Hcls] ]";[solve_ndisj|solve_ndisj|].
+        iDestruct (big_sepL2_length with "Hprog'") as %Hlength_rest'. 
+        iMod (na_inv_open with "Hbec Hown") as "[Hbec' [Hown Hcls'] ]";[solve_ndisj|solve_ndisj|].
+        iApply (scall_epilogue_spec with "[- $HPC $Hbec' $Hr_t1 $Hr_t2]");[|apply Hnext|]. 
+        { split;auto. }
+        iNext. iIntros "(HPC & Hr_t1 & Hr_t2 & Hbec')".
+        iMod ("Hcls'" with "[$Hbec' $Hown]") as "Hown". 
+        iDestruct "Hr_t1" as (wrt1') "Hr_t1".
 
-    (* All we need to do is to uninitialize the adversary stack *)
-    rewrite /W' std_update_multiple_revoke_commute; auto.
-    iDestruct (big_sepL_sep with "Hstackrest") as "[Hstackrest _]".
-    iDestruct (big_sepL_sep with "Hstackrest") as "[Hstackrest Hstackrest']".
-    iDestruct (region_addrs_exists with "Hstackrest") as (wsrest) "Hstackrest".
-    iDestruct (big_sepL2_length with "Hstackrest") as %Hlengthstackrest.
-    iDestruct (big_sepL2_to_big_sepL_l with "Hstackrest'") as "Hstackrest'"; [eapply Hlengthstackrest|].
-    iDestruct (big_sepL2_sep with "[$Hstackrest $Hstackrest']") as "Hstackrest".
-    set m_uninit1 : gmap Addr Word := list_to_map (zip ltemprest wsrest).
-    iMod (region_revoked_to_uninitialized _ m_uninit1 with "[$Hsts $Hr Hstackrest]") as "[Hsts Hr]".
-    { iDestruct (big_sepL2_to_big_sepM with "Hstackrest") as "HH".
-      - eapply NoDup_filter, NoDup_ListNoDup, NoDup_ListNoDup, region_addrs_NoDup.
-      - rewrite /m_uninit1. iApply (big_sepM_mono with "HH").
-        simpl; intros. iIntros "[(A & B & C & D) E]".
-        iExists _, _. iFrame. iPureIntro. intros; eapply interp_persistent. }
+        (* Since there is just one local register, it is easier to just step through rather than using the macro spec *)
+        rewrite /restore_locals_instrs.
+        destruct ai_rest';[inversion Hlength_rest'|]. apply contiguous_between_cons_inv_first in Hcont_rest' as Heq;subst a3.
+        destruct ai_rest';[inversion Hlength_rest'|].
+        iRename "Hprog" into "Hprog_inv".
+        (* lea r_t2 -1 *)
+        iPrologue "Hprog'".
+        iMod (na_inv_open with "Hbel Hown") as "[>Hbel' [Hown Hcls'] ]";[solve_ndisj|solve_ndisj|].
+        iDestruct (big_sepL2_length with "Hbel'") as %Hbl_length. 
+        assert ((b_l + 1) = Some e_l)%a as Hbl_next. 
+        { rewrite region_addrs_length /= /region_size in Hbl_length. clear -Hbl_length. solve_addr. }
+        assert ((e_l + -1)%a = Some b_l) as Hlea.
+        { clear -Hbl_next. solve_addr. }
+        iApply (wp_lea_success_z with "[$HPC $Hi $Hr_t2]");
+          [apply decode_encode_instrW_inv|iCorrectPC a_call_end a_last|iContiguous_next Hcont_rest' 0|apply Hlea|auto|..]. 
+        iEpilogue "(HPC & Hprog_done & Hr_t2)". 
+        (* load r_env r_t2 *)
+        apply region_addrs_single in Hbl_next.
+        rewrite /region_mapsto Hbl_next.
+        iDestruct "Hbel'" as "[Hbel' _]".
+        destruct ai_rest';[inversion Hlength_rest'|].
+        iPrologue "Hprog".
+        iAssert (⌜(b_l =? a3)%a = false⌝)%I as %Hfalse.
+        { destruct (decide (b_l = a3)%Z); [subst|iPureIntro;apply Z.eqb_neq,neq_z_of;auto].
+          iDestruct (mapsto_valid_2 with "Hi Hbel'") as %?. done. }
+        iApply (wp_load_success with "[$HPC $Hi $Hr_env $Hr_t2 Hbel']");
+          [apply decode_encode_instrW_inv|iCorrectPC a_call_end a_last| |iContiguous_next Hcont_rest' 1|..]. 
+        { split;auto. rewrite andb_true_iff Z.leb_le Z.ltb_lt. clear -Hlea. solve_addr. }
+        { rewrite Hfalse. iFrame. }
+        rewrite Hfalse. iEpilogue "(HPC & Hr_env & Hi & Hr_t2 & Hb_l)". iCombine "Hi" "Hprog_done" as "Hprog_done".
+        (* load r_env r_t0 *)
+        destruct ai_rest';[inversion Hlength_rest'|].
+        iPrologue "Hprog".
+        iInv (logN.@b) as (wd) ">[Hd %]" "Hcls''". subst wd. 
+        iAssert (⌜(b =? a4)%a = false⌝)%I as %Hfalse'.
+        { destruct (decide (b = a4)%Z); [subst|iPureIntro;apply Z.eqb_neq,neq_z_of;auto].
+          iDestruct (mapsto_valid_2 with "Hi Hd") as %?. done. }
+        iApply (wp_load_success with "[$HPC $Hi $Hr_t0 $Hr_env Hd]");
+          [apply decode_encode_instrW_inv|iCorrectPC a_call_end a_last| |iContiguous_next Hcont_rest' 2|..]. 
+        { split;auto. rewrite andb_true_iff Z.leb_le Z.ltb_lt. clear -Hincr. solve_addr. }
+        { rewrite Hfalse'. iFrame. } rewrite Hfalse'.
+        iNext. iIntros "(HPC & Hr_t0 & Hi & Hr_env & Hd)". iCombine "Hi" "Hprog_done" as "Hprog_done".
+        iMod ("Hcls''" with "[Hd]") as "_".
+        { iNext. iExists _. iFrame. auto. }
+        iModIntro. iApply wp_pure_step_later;auto;iNext.
 
-    assert (Heqq: region_addrs a asplit = (a :: stack_own_b :: stack_own)).
-    { rewrite -region_addrs_length Hstack_eq1 app_length Hlength_own in Hspliteq.
-      rewrite Hstack_eq1. destruct stack_adv; [rewrite app_nil_r; auto|].
-      simpl in Hspliteq; lia. }
-    assert (Hxx: stack_own_last = asplit).
-    { assert (a <= asplit)%a.
-      { revert Hspliteq. clear. intros.
-        rewrite /region_size in Hspliteq. solve_addr. }
-      revert Hstack_own_bound Hspliteq H Heqq.
-      rewrite -region_addrs_length. clear.
-      simpl. intros. symmetry in Heqq.
-      generalize (contiguous_between_of_region_addrs _ _ _ H Heqq).
-      intro. inversion H0; subst. inv H6. 
-      assert ((a + 8)%a = Some stack_own_last) by solve_addr.
-      rewrite region_addrs_length in Hspliteq.
-      generalize (contiguous_between_of_region_addrs_aux _ _ stack_own_last _ Heqq).
-      rewrite Hspliteq. rewrite H1. intro.
-      generalize (H2 eq_refl); clear H2; intro.
-      revert H0 H2; clear; intros. eapply contiguous_between_inj; eauto. }
-    subst asplit.
-    (* Resulting world *)
-    set W'' := (override_uninitializedW m_uninit1 (revoke (std_update_multiple W luninitsplit Revoked))).
-    
-    assert (related_sts_priv_world W W'') as HWW''.
-    { eapply related_sts_priv_trans_world with W'; auto.
-      - eapply related_sts_priv_trans_world;[apply revoke_related_sts_priv;auto|].
-        rewrite /W'. eapply related_sts_priv_world_std_update_multiple.
-        eapply Forall_forall. intros.
-        eapply Forall_forall in Huninit; eauto.
-        destruct Huninit. exists (Static {[x:=x0]}).
-        split; auto. rewrite revoke_monotone_lookup_same'; auto.
-        rewrite H0; auto.
-      - rewrite /W' /W''. rewrite -std_update_multiple_revoke_commute;auto.
-        apply related_sts_priv_world_override_uninitializedW.
-        eapply Forall_forall. intros.
-        eapply (proj1 (elem_of_elements _ _)) in H.
-        eapply elem_of_dom in H. destruct H.
-        eapply elem_of_list_to_map_2, elem_of_zip_l, elem_of_list_filter in H as [Htempx Hx].
-        assert (x ∉ luninitsplit) as Hnin.
-        { intros Hcontr. eapply Forall_forall in Huninit;eauto. destruct Huninit as [? Huninit].
-          rewrite Htempx in Huninit. congruence. }
-        rewrite std_sta_update_multiple_lookup_same_i;auto.
-        exists Revoked. rewrite revoke_lookup_Temp;auto. 
-    }
-
-    iAssert (⌜Forall (λ a, region_type_uninitialized W a ∨ region_type_temporary W a) (region_addrs a e_r)⌝)%I as %HWstates.
-    { rewrite Forall_forall. iIntros (x Hx).
-      iDestruct (big_sepL_elem_of _ _ x with "Hstk_val") as (? ?) "[_ [H | H] ]";auto;[iRight;auto|iLeft;auto]. }
-
-    assert (forall x, x ∈ region_addrs stack_own_last e_r -> region_type_uninitialized W'' x) as HrestpwlU.
-    { intros x Hx.
-      rewrite /W''.
-      destruct (m_uninit1 !! x) eqn:Hsome. 
-      - exists w1. apply override_uninitializedW_lookup_some;auto.
-      - rewrite /region_type_uninitialized. rewrite override_uninitializedW_lookup_none;auto.
-        apply withinBounds_le_addr in Hwb2.
-        assert (x ∈ region_addrs a e_r) as Hbe.
-          { rewrite (region_addrs_split _ stack_own_last);[apply elem_of_app;by right|
-                                                          revert Hwb2;clear;solve_addr]. }
-        assert (x ∉ luninitsplit) as Hnin.
-        { intros Hcontr%elem_of_list_filter. destruct Hcontr as [_ Hcontr].
-          apply (region_addrs_xor_elem_of _ _ stack_own_last) in Hbe as [ [? ?] | [? ?] ];try done. }
-        rewrite -std_update_multiple_revoke_commute;auto.
-        rewrite std_sta_update_multiple_lookup_same_i;auto.
-        assert (W.1 !! x ≠ Some Temporary) as Hntemp.
-        { intros Hcontr. apply not_elem_of_list_to_map in Hsome. apply Hsome. 
-          rewrite fst_zip;[|rewrite Hlengthstackrest;clear;lia]. 
-          apply elem_of_list_filter. split;auto. }
-        revert HWstates. rewrite Forall_forall =>HWstate. apply HWstate in Hbe. 
-        destruct Hbe as [ [? ?] | Hcontr];[|done]. 
-        exists x0. rewrite revoke_monotone_lookup_same;auto.
-    }
-    
-    (* We choose the current register state *)
-    set (r := <[PC    := inl 0%Z]>
-                     (<[r_stk := inr (URWLX, Local, stack_own_last, e_r, stack_own_last)]>
-                     (<[r_t0  := inr (E, Local, a, stack_own_last, stack_own_b)]>
-                     (<[r_t30 := wadv]>
-                     (create_gmap_default
-                        (list_difference all_registers [PC; r_stk; r_t0; r_t30]) (inl 0%Z)))))).
-    
-    (* We now want to apply the jmp or fail pattern of wadv *)
-    iDestruct (jmp_or_fail_spec _ _ φ with "Hadv") as "Hadv_cont".
-    
-    (* jmp r_adv *)
-    iDestruct (big_sepL2_length with "Hf2") as %Hrest_length; simpl in Hrest_length. 
-    destruct rest;[inversion Hrest_length|].
-    iPrologue rest Hrest_length "Hf2".
-    apply contiguous_between_cons_inv_first in Hcont_rest as Heq. subst a0. 
-    iApply (wp_jmp_success with "[$Hinstr $Hr_adv $HPC]");
-      [apply decode_encode_instrW_inv|apply Hfl|iCorrectPC s_last a_last|..].
-    (* before applying the epilogue, we want to distinguish between a correct or incorrect resulting PC *)
-    destruct (decide (isCorrectPC (updatePcPerm wadv))). 
-    2: { iEpilogue "(HPC & _ & _)". iApply ("Hadv_cont" with "[Hφ $HPC]").
-         iApply "Hφ". iIntros (Hcontr). done. }
-    iDestruct "Hadv_cont" as (p g b e a0 Heq) "Hadv_cont". symmetry in Heq. simplify_eq.
-    destruct g;inversion Hglobal. 
-    iDestruct ("Hadv_cont" $! r _ HWW'') as "Hadv_contW''". 
-    iEpilogue "(HPC & Hinstr & Hr_adv)". iSimpl in "HPC".
-
-    (* We have now arrived at the interesting part of the proof: namely the unknown 
-       adversary code. In order to reason about unknown code, we must apply the 
-       fundamental theorem. To this purpose, we must first define the stsf that will 
-       describe the behavior of the memory. *)
-
-    (* We have all the resources of r *)
-    iAssert (registers_mapsto (<[PC:=match p with
-                                     | E => inr (RX, Global, b, e, a0)
-                                     | _ => inr (p, Global, b, e, a0)
-                                     end]> r))
-                          with "[Hr_gen Hr_stk Hr_t0 Hr_adv HPC]" as "Hmaps".
-    { iApply (registers_mapsto_resources with "[$Hr_gen] [$Hr_stk] [$Hr_t0] [$Hr_adv] [$HPC]").
-      rewrite !dom_delete_L Hrmap_dom. clear. set_solver. }
-    (* r contrains all registers *)
-    iAssert (full_map r) as "#full";[iApply r_full|].
-    (* Need to prove the validity of the continuation, the stack, as well as put
-       local memory into invariant. *)
-    iMod (na_inv_alloc logrel_nais ⊤ (nroot.@"Hprog") with "Hprog")%I as "#Hprog".
-    iMod (na_inv_alloc logrel_nais ⊤ (nroot.@"Hframe") _ with "Hstack_own") as "#Hlocal".
-    iMod (na_inv_alloc logrel_nais ⊤ (nroot.@"Hlink") with "Hlink") as "#Hlink". 
-    (* We will put the local state 1 into a separate invariant *)
-    iMod (na_inv_alloc logrel_nais ⊤ (nroot.@"local") with "Hb_r")%I as "#Hlocal_one".
-    iAssert (∀ r1 : RegName, ⌜r1 ≠ PC⌝ → (fixpoint interp1) W'' (r !r! r1))%I
-      with "[-Hsts Hmaps Hna Hφ Hr]" as "Hreg".
-    { iIntros (r1).
-      assert (r1 = PC ∨ r1 = r_stk ∨ r1 = r_t0 ∨ r1 = r_t30 ∨ (r1 ≠ PC ∧ r1 ≠ r_stk ∧ r1 ≠ r_t0 ∧ r1 ≠ r_t30)) as Hne.
-      { destruct (decide (r1 = PC)); [by left|right].
-        destruct (decide (r1 = r_stk)); [by left|right].
-        destruct (decide (r1 = r_t0)); [by left|right].
-        destruct (decide (r1 = r_t30)); [by left|right;auto].  
-      }
-      destruct Hne as [-> | [-> | [-> | [Hr_t30 | [Hnpc [Hnr_stk [Hnr_t0 Hnr_t30] ] ] ] ] ] ].
-      - iIntros "%". contradiction.
-      - (* invariant for the stack of the adversary *)
-        assert (r !! r_stk = Some (inr (URWLX, Local, stack_own_last, e_r, stack_own_last))) as Hr_stk; auto. 
-        rewrite /RegLocate Hr_stk !fixpoint_interp1_eq. 
-        iIntros (_). iSimpl.
-        assert (Hmin1: min stack_own_last e_r = stack_own_last).
-        { apply withinBounds_le_addr in Hwb2. revert Hwb2. clear. solve_addr. }
-        rewrite !Hmin1. replace (max stack_own_last stack_own_last) with stack_own_last by (clear; solve_addr).
-        rewrite (region_addrs_empty stack_own_last stack_own_last); [|clear; solve_addr].
-        rewrite big_sepL_nil. iSplitR;[auto|].
-        iApply big_sepL_forall. iIntros (k x Hx).
-        assert (x ∈ region_addrs a e_r) as Hin.
-        { apply withinBounds_le_addr in Hwb2.
-          rewrite (region_addrs_split _ stack_own_last);[|revert Hwb2;clear;solve_addr].
-          apply elem_of_app. right. apply elem_of_list_lookup. eauto. }
-        iDestruct (big_sepL_elem_of _ _ x with "Hstk_val") as (p' Hfl') "[Hx _]";[auto|].
-        destruct p';inversion Hfl'.
-        iExists RWLX. iFrame "Hx". iSplit;[auto|]. iPureIntro. right. apply HrestpwlU.
-        apply elem_of_list_lookup. eauto. 
-      - (* continuation *)
-        iIntros (_). 
-        assert (r !! r_t0 = Some (inr (E, Local, a, stack_own_last, stack_own_b))) as Hr_t0; auto. 
-        rewrite /RegLocate Hr_t0 !fixpoint_interp1_eq. iSimpl. 
-        (* prove continuation *)
-        (* iExists _,_,_,_. iSplit;[eauto|]. *)
-        iAlways.
-        rewrite /enter_cond. 
-        iIntros (r' W2 HWW2).
-        iNext. iSimpl. 
-        (* iExists _,_.  do 2 (iSplit; [eauto|]).*)
-        iIntros "(#[Hfull' Hreg'] & Hmreg' & Hr & Hs & Hna)". 
-        iSplit; [auto|rewrite /interp_conf].
-        (* get the PC, currently pointing to the activation record *)
-        iDestruct (big_sepM_delete _ _ PC with "Hmreg'") as "[HPC Hmreg']";[rewrite lookup_insert; eauto|].
-        (* get a general purpose register *)
-        iAssert (⌜∃ wr_t1, r' !! r_t1 = Some wr_t1⌝)%I as %[rt1w Hrt1];
-          first iApply "Hfull'".
-        iDestruct (big_sepM_delete _ _ r_t1 with "Hmreg'") as "[Hr_t1 Hmreg']".
-        { rewrite lookup_delete_ne; auto.
-          rewrite lookup_insert_ne; eauto. }
-        (* get r_stk *)
-        iAssert (⌜∃ wr_stk, r' !! r_stk = Some wr_stk⌝)%I as %[rstkw Hrstk];
-          first iApply "Hfull'".
-        iDestruct (big_sepM_delete _ _ r_stk with "Hmreg'") as "[Hr_stk Hmreg']".
-        { do 2 (rewrite lookup_delete_ne; auto).
-          rewrite lookup_insert_ne; eauto. }
-        (* get r_t30 *)
-        iAssert (⌜∃ wr30, r' !! r_t30 = Some wr30⌝)%I as %[wr30 Hr30];
-          first iApply "Hfull'".
-        iDestruct (big_sepM_delete _ _ r_t30 with "Hmreg'") as "[Hr_t30 Hmreg']".
-        { do 3 (rewrite lookup_delete_ne; auto).
-          rewrite lookup_insert_ne; eauto. }
-        (* open the na invariant for the local stack content *)
-        iMod (na_inv_open logrel_nais ⊤ ⊤ with "Hlocal Hna") as "(>Hframe & Hna & Hcls)";auto. 
-        assert (PermFlows RX RWLX) as Hrx;[by rewrite /PermFlows /=|].
-        (* prepare the continuation *)
-        let a := fresh "a" in destruct rest as [|a rest];[inversion Hf2_length|].
-        (* prepare the new stack value *)
-        assert (exists stack_new, (stack_new + 1)%a = Some stack_own_end) as [stack_new Hstack_new].
-        { revert Hstack_own_bound'. clear. intros H. destruct (stack_own_b + 5)%a eqn:Hsome;[|solve_addr].
-          exists a. solve_addr. }
-        assert (withinBounds (URWLX, Local, a, e_r, stack_own_end) = true) as Hwb3.
-        { isWithinBounds. 
-          - assert ((a + 1)%a = Some stack_own_b) as Hincr;[apply contiguous_between_incr_addr with (i := 1) (ai := stack_own_b) in Hcont1; auto|].
-            revert Hstack_own_bound' Hincr. clear. solve_addr. 
-          - apply withinBounds_le_addr in Hwb2 as [_ Hwb2]. revert Hstack_own_bound Hstack_own_bound' Hwb2. clear. solve_addr. 
-        }
-        (* step through instructions in activation record *)
-        iApply (scallU_epilogue_spec with "[-]"); last iFrame "Hframe HPC Hr_t1 Hr_stk";auto;
-          [|iContiguous_next Hcont_rest 0|apply Hstack_new|..]. 
-        { intros mid Hmid. split;[|auto]. apply withinBounds_le_addr in Hwb2.
-          apply (contiguous_between_middle_bounds _ 1 stack_own_b) in Hcont1;[|auto]. revert Hwb2 Hcont1 Hmid. clear. solve_addr.
-        }
-        { revert Hstack_own_bound Hstack_own_bound';clear;solve_addr. }
-        iNext. iIntros "(HPC & Hr_stk & Hr_t1 & Hframe)".
-        iDestruct "Hr_t1" as (wrt1) "Hr_t1". 
-        (* we don't want to close the stack invariant yet, as we will now need to pop it *)
-        (* go through rest of the program. We will now need to open the invariant one instruction at a time *)
-        (* sub r_t1 0 7 *)
-        iPrologue_pre rest Hf2_length. 
-        iMod (na_inv_open with "Hprog Hna") as "[ [>Hinstr Hprog_rest] [Hna Hcls'] ]";[solve_ndisj..|].
-        iApply (wp_add_sub_lt_success_z_z with "[$HPC $Hr_t1 $Hinstr]");
-          [apply decode_encode_instrW_inv|right;left;eauto|iContiguous_next Hcont_rest 1|apply Hfl|iCorrectPC s_last a_last|..]. 
-        iNext. iIntros "(HPC & Hinstr & Hr_t1)".
-        iMod ("Hcls'" with "[$Hna $Hinstr $Hprog_rest]") as "Hna".
-        iApply wp_pure_step_later;auto;iNext.
-        (* lea r_stk r_t1 *) 
-        iPrologue_pre rest Hf2_length. 
-        iMod (na_inv_open with "Hprog Hna") as "[(Ha79 & >Ha80 & Hprog_rest) (Hna & Hcls')]";[solve_ndisj..|].
-        assert ((stack_own_end + (0 - 6))%a = Some stack_own_b) as Hpop.
-        { revert Hstack_own_bound' Hstack_new. clear. solve_addr. }
-        iApply (wp_lea_success_reg with "[$HPC $Hr_t1 $Hr_stk $Ha80]");
-          [apply decode_encode_instrW_inv|apply Hfl|iCorrectPC s_last a_last|iContiguous_next Hcont_rest 2|apply Hpop|auto..].
-        { simpl. revert Hpop;clear;solve_addr. }
-        iNext. iIntros "(HPC & Ha80 & Hr_t1 & Hr_stk)".
-        iMod ("Hcls'" with "[$Hna $Ha79 $Ha80 $Hprog_rest]") as "Hna".
-        iApply wp_pure_step_later;auto;iNext.
-        (* pop r_stk *)
-        iMod (na_inv_open with "Hprog Hna") as "[(Ha79 & Ha80 & >Hprog_rest) (Hna & Hcls')]";[solve_ndisj..|].
-        iMod (na_inv_open with "Hlocal_one Hna") as "[>Hb_r [Hna Hcls''] ]";[solve_ndisj..|].
-        do 2 (destruct rest;[by inversion Hlength_f2|]). 
-        iDestruct (mapsto_decomposition [a4;a5;a6] _ _ (popU_instrs r_stk r_t30) with "Hprog_rest") as "[Hpop Hprog_rest]";
-          [auto|]. 
-        iApply (popU_spec with "[-]"); last iFrame "Hpop Hr_t30 Hr_stk HPC Hr_t1 Hb_r";
-          [split; [|split]; iCorrectPC s_last a_last|apply Hfl|auto| |auto|iContiguous_next Hcont_rest 3|
-           iContiguous_next Hcont_rest 4|iContiguous_next Hcont_rest 5|iContiguous_next Hcontiguous' 0|..].
-        { apply le_addr_withinBounds. clear. solve_addr. revert Hsize;clear;rewrite /region_size. solve_addr. }
-        iNext. iIntros "(HPC & Hpop & Hr_t30 & Hb_r & Hr_stk & Hr_t1)". 
-        iMod ("Hcls''" with "[$Hna $Hb_r]") as "Hna". 
-        iMod ("Hcls'" with "[$Hna $Ha79 $Ha80 Hpop Hprog_rest]") as "Hna".
-        { iApply (big_sepL2_app with "Hpop [-]"). iFrame. }
+        (* prepare memory for the assert macro *)
+        iDestruct (contiguous_between_program_split with "Hprog") as
+        (ai_assert ai_rest'' a_assert_end) "(Hassert_prog & Hprog & #Hcont)".
+        { repeat (apply contiguous_between_cons_inv in Hcont_rest' as [_ [? [_ Hcont_rest'] ] ];
+                  apply contiguous_between_cons_inv_first in Hcont_rest' as Heq'; subst x). apply Hcont_rest'. }
+        iDestruct "Hcont" as %(Hcont_assert & Hcont_rest'' & Heqapp'' & Hlink'').
+        iDestruct (big_sepL2_length with "Hassert_prog") as %Hai_assert_len.
+        assert (isCorrectPC_range pc_p pc_b pc_e a5 a_assert_end) as Hvpc5.
+        { eapply isCorrectPC_range_restrict. apply Hvpc.
+          generalize (contiguous_between_bounds _ _ _ Hcont_rest').
+          generalize (contiguous_between_bounds _ _ _ Hcont_rest'').
+          generalize (contiguous_between_bounds _ _ _ Hcont_malloc).
+          generalize (contiguous_between_bounds _ _ _ Hcont_call).
+          apply contiguous_between_middle_bounds' with (ai:=a5) in Hcont_rest';[|repeat constructor].
+          apply contiguous_between_middle_bounds' with (ai:=a2) in Hcont_rest;[|repeat constructor].
+          clear -Hcont_rest' Hcont_rest. solve_addr. }
+        assert (isCorrectPC_range pc_p pc_b pc_e a_assert_end a_last) as Hvpc6.
+        { eapply isCorrectPC_range_restrict. apply Hvpc.
+          generalize (contiguous_between_bounds _ _ _ Hcont_rest').
+          generalize (contiguous_between_bounds _ _ _ Hcont_rest'').
+          generalize (contiguous_between_bounds _ _ _ Hcont_malloc).
+          generalize (contiguous_between_bounds _ _ _ Hcont_call).
+          apply contiguous_between_middle_bounds' with (ai:=a5) in Hcont_rest';[|repeat constructor].
+          apply contiguous_between_middle_bounds' with (ai:=a2) in Hcont_rest;[|repeat constructor].
+          clear -Hcont_rest' Hcont_rest Hlink''. solve_addr. }
         
-        (* we will not use the local stack anymore, so we may close the na_inv *)
-        iMod ("Hcls" with "[$Hframe $Hna]") as "Hna".
+        (* assert macro *)
+        iMod (na_inv_open with "Hlink Hown") as "[ (a_entry' & a_env & >pc_b & >Ha_entry) [Hown Hcls''] ]";[solve_ndisj..|]. 
+        iApply (assert_r_z_success with "[- $HPC $Hassert_prog $pc_b $a_entry' $Hr_t0]");
+          [apply Hvpc5|apply Hcont_assert|auto..].
+        iSplitL "Hr_t1";[eauto|]. 
+        iSplitL "Hr_t2";[eauto|].
+        iSplitL "Hr_t3";[eauto|]. 
+        iNext. iIntros "(Hr_t1 & Hr_t2 & Hr_t3 & Hr_t0 & HPC & Hassert_prog & Hpc_b & Ha_entry')".
+        iMod ("Hcls''" with "[$Hown $Ha_entry' $a_env $Hpc_b $Ha_entry]") as "Hown".
+        iMod ("Hcls'" with "[$Hown $Hb_l]") as "Hown";[iNext;done|].  
 
-        (* we will now make the assertion that r_t30 points to 1 *)
-        iAssert (⌜∃ w, r' !! r_t2 = Some w⌝)%I as %[w2 Hr2]; first iApply "Hfull'".
-        iDestruct (big_sepM_delete _ _ r_t2 with "Hmreg'") as "[Hr_t2 Hmreg']".
-        { do 4 (rewrite lookup_delete_ne; auto). rewrite lookup_insert_ne; eauto. }
-        iAssert (⌜∃ w, r' !! r_t3 = Some w⌝)%I as %[w3 Hr3]; first iApply "Hfull'".
-        iDestruct (big_sepM_delete _ _ r_t3 with "Hmreg'") as "[Hr_t3 Hmreg']".
-        { do 5 (rewrite lookup_delete_ne; auto). rewrite lookup_insert_ne; eauto. }
-        iMod (na_inv_open with "Hprog Hna") as "[(Ha79 & Ha80 & >Hprog_rest) (Hna & Hcls')]";[solve_ndisj..|].
-        iDestruct (mapsto_decomposition [a4;a5;a6] _ _ (popU_instrs r_stk r_t30) with "Hprog_rest") as "[Hpop Hprog_rest]";
-          [auto|].
-        iDestruct (big_sepL2_length with "Hprog_rest") as %Hlength_rest.
-        assert (contiguous_between (a7 :: rest) a7 a_last) as Hcont_rest_weak.
-        { repeat (inversion Hcont_rest as [|????? Hcont_rest']; subst; auto; clear Hcont_rest; rename Hcont_rest' into Hcont_rest). }
-        iDestruct (contiguous_between_program_split with "Hprog_rest") as (rest1 rest2 link0) "(Hassert & Hhalt & #Hcont)";
-          [apply Hcont_rest_weak|].
-        iDestruct "Hcont" as %(Hcont_rest1 & Hcont_rest2 & Heq_app1 & Hlink0).
-        iDestruct (big_sepL2_length with "Hhalt") as %Hrest2.
-        destruct rest2;[inversion Hrest2|].
-        apply contiguous_between_cons_inv_first in Hcont_rest2 as Heq. subst a8. 
-        iMod (na_inv_open with "Hlink Hna") as "[ [>Hpc_b >Ha_entry] [Hna Hcls''] ]";[solve_ndisj..|]. 
-        iApply (assert_r_z_success with "[-]");last iFrame "Hassert HPC Hr_t30 Hpc_b Ha_entry";auto;[|apply Hcont_rest1|].
-        { intros mid Hmid. apply isCorrectPC_inrange with s_last a_last; auto.
-          apply contiguous_between_middle_bounds with (i:=6) (ai:=a7) in Hcont_rest;auto.
-          apply contiguous_between_middle_bounds with (i:=0) (ai:=link0) in Hcont_rest2;auto.
-          revert Hmid Hcont_rest Hcont_rest2. clear. solve_addr. }
-        iSplitL "Hr_t1";[iNext;iExists _;iFrame|].
-        iSplitL "Hr_t2";[iNext;iExists _;iFrame|].
-        iSplitL "Hr_t3";[iNext;iExists _;iFrame|].
-        iNext. iIntros "(Hr_t1 & Hr_t2 & Hr_t3 & Hr_t30 & HPC & Hassert & Hpc_b & Ha_entry)". 
-        iMod ("Hcls''" with "[$Hna $Hpc_b $Ha_entry]") as "Hna".
         (* halt *)
-        destruct rest2;[|inversion Hrest2].
-        apply contiguous_between_last with (ai:=link0) in Hcont_rest2 as Hlast;auto. 
-        iApply (wp_bind (fill [SeqCtx])).
-        iDestruct "Hhalt" as "[Hinstr _]". 
-        iApply (wp_halt with "[$HPC $Hinstr]");
-          [apply decode_encode_instrW_inv|apply Hfl| |].
-        { apply isCorrectPC_inrange with s_last a_last; auto.
-          apply contiguous_between_middle_bounds with (i:=6) (ai:=a7) in Hcont_rest as Hle;auto.
-          apply contiguous_between_bounds in Hcont_rest.
-          apply contiguous_between_bounds in Hcont_rest1. 
-          revert Hcont_rest Hcont_rest1 Hle Hlast. clear. solve_addr. }
-        iNext. iIntros "(HPC & Hinstr)".
-        iMod ("Hcls'" with "[$Hna Ha79 Ha80 Hpop Hassert Hinstr]") as "Hna".
-        { iNext. iFrame "Ha79 Ha80".
-          iApply (big_sepL2_app with "Hpop [-]"). rewrite Heq_app1.
-          iApply (big_sepL2_app with "Hassert [-]"). iFrame. done. }
-        iApply wp_pure_step_later;auto;iNext.
-        (* halted: need to show post condition *)
-        iApply wp_value. iIntros "_".
-        evar (r'' : gmap RegName Word).
-        instantiate (r'' := <[PC    := inr (pc_p, pc_g, pc_b, pc_e, link0)]>
-                           (<[r_t1  := inl 0%Z]>
-                           (<[r_t2  := inl 0%Z]>
-                           (<[r_t3  := inl 0%Z]>
-                           (<[r_t30 := inl 0%Z]>
-                           (<[r_stk := inr (URWLX, Local, a, e_r, a)]> r')))))). 
-        iFrame. iExists r'',_. iFrame. iSplit;[|iSplit].
-        + iDestruct "Hfull'" as %Hfull'.
-          iPureIntro.
-          intros r0. rewrite /r''.
-          destruct (decide (PC = r0));first subst. 
-          { rewrite lookup_insert. eauto. }
-          rewrite lookup_insert_ne; auto. 
-          destruct (decide (r_t1 = r0));first subst. 
-          { rewrite lookup_insert. eauto. }
-          rewrite lookup_insert_ne; auto. 
-          destruct (decide (r_t2 = r0));first subst. 
-          { rewrite lookup_insert. eauto. }
-          rewrite lookup_insert_ne; auto.
-          destruct (decide (r_t3 = r0));first subst. 
-          { rewrite lookup_insert. eauto. }
-          rewrite lookup_insert_ne; auto.
-          destruct (decide (r_t30 = r0));first subst. 
-          { rewrite lookup_insert. eauto. }
-          rewrite lookup_insert_ne; auto. 
-          destruct (decide (r_stk = r0));first subst. 
-          { rewrite lookup_insert. eauto. }
-          rewrite lookup_insert_ne; auto.
-        + rewrite /r''.
-          iDestruct (big_sepM_delete (λ x y, x ↦ᵣ y)%I r'' PC
-                       with "[-]") as "Hmreg'"; auto.
-          { by rewrite lookup_insert. }
-          iFrame. do 2 rewrite delete_insert_delete.
-          iDestruct (big_sepM_delete (λ x y, x ↦ᵣ y)%I _ r_t1
-                       with "[-]") as "Hmreg'"; auto.
-          { rewrite lookup_delete_ne; auto. by rewrite lookup_insert. }
-          iFrame. do 2 rewrite (delete_commute _ r_t1 PC).
-          rewrite delete_insert_delete.
-          do 2 rewrite (delete_commute _ PC r_t1).
-          iDestruct (big_sepM_delete (λ x y, x ↦ᵣ y)%I _ r_t2
-                       with "[-]") as "Hmreg'"; auto.
-          { repeat (rewrite lookup_delete_ne; auto). by rewrite lookup_insert. }
-          iFrame. repeat rewrite (delete_commute _ r_t2 _). rewrite delete_insert_delete. 
-          iDestruct (big_sepM_delete (λ x y, x ↦ᵣ y)%I _ r_t3
-                       with "[-]") as "Hmreg'"; auto.
-          { repeat (rewrite lookup_delete_ne; auto). by rewrite lookup_insert. }
-          iFrame. repeat rewrite (delete_commute _ r_t3 _). rewrite delete_insert_delete. 
-          iDestruct (big_sepM_delete (λ x y, x ↦ᵣ y)%I _ r_t30
-                       with "[-]") as "Hmreg'"; auto.
-          { repeat (rewrite lookup_delete_ne; auto). by rewrite lookup_insert. }
-          iFrame. repeat rewrite (delete_commute _ r_t30 _). rewrite delete_insert_delete. 
-          iDestruct (big_sepM_delete (λ x y, x ↦ᵣ y)%I _ r_stk
-                       with "[-]") as "Hmreg'"; auto.
-          { repeat (rewrite lookup_delete_ne; auto). by rewrite lookup_insert. }
-          iFrame. repeat rewrite (delete_commute _ r_stk _). rewrite delete_insert_delete. 
-          iFrame.           
-        + iPureIntro. apply related_sts_priv_refl_world. 
-      - rewrite Hr_t30. 
-        assert (r !! r_t30 = Some (inr (p, Global, b, e, a0))) as Hr_t30_some; auto.
-        iIntros (_). iApply (interp_monotone_nl with "[] [] Hadv");auto. 
-      - (* in this case we can infer that r1 points to 0, since it is in the list diff *)
-        assert (r !r! r1 = inl 0%Z) as Hr1.
-        { rewrite /RegLocate.
-          destruct (r !! r1) eqn:Hsome; rewrite Hsome; last done. rewrite /r in Hsome. 
-          do 4 (rewrite lookup_insert_ne in Hsome;auto). 
-          assert (Some s = Some (inl 0%Z)) as Heq.
-          { rewrite -Hsome. apply create_gmap_default_lookup.
-            apply elem_of_list_difference. split; first apply all_registers_correct.
-            repeat (apply not_elem_of_cons;split;auto).
-            apply not_elem_of_nil. 
-          }
-          by inversion Heq. 
-        }
-        rewrite Hr1 !fixpoint_interp1_eq. iSimpl. auto. 
+        iDestruct (big_sepL2_length with "Hprog") as %Hlength_rest''. 
+        destruct ai_rest'';[inversion Hlength_rest''|]. destruct ai_rest'';[|inversion Hlength_rest'']. 
+        apply contiguous_between_cons_inv_first in Hcont_rest'' as Heq; subst a6. 
+        iPrologue "Hprog". 
+        iApply (wp_halt with "[$HPC $Hi]");
+          [apply decode_encode_instrW_inv|iCorrectPC a_assert_end a_last|..].
+        iEpilogue "(HPC & Hi)".
+
+        (* reassemble registers, close invariants and finish *)
+        iMod ("Hcls" with "[$Hown Hprog_done Hi Hassert_prog]") as "Hown". 
+        { iNext. iDestruct "Hprog_done" as "($&$&$)".
+          rewrite Heqapp''. iApply (big_sepL2_app with "Hassert_prog [Hi]"). iFrame. done. }
+        iDestruct (big_sepM_insert with "[$Hreg $Hr_t3]") as "Hreg";[apply lookup_delete|rewrite insert_delete -delete_insert_ne//].
+        iDestruct (big_sepM_insert with "[$Hreg $Hr_t0]") as "Hreg";[apply lookup_delete|rewrite insert_delete -!delete_insert_ne//].
+        iDestruct (big_sepM_insert with "[$Hreg $Hr_env]") as "Hreg";[apply lookup_delete|rewrite insert_delete -!delete_insert_ne//].
+        iDestruct (big_sepM_insert with "[$Hreg $Hr_t2]") as "Hreg";[apply lookup_delete|rewrite insert_delete -!delete_insert_ne//].
+        iDestruct (big_sepM_insert with "[$Hreg $Hr_t1]") as "Hreg";[apply lookup_delete|rewrite insert_delete -!delete_insert_ne//].
+        iDestruct (big_sepM_insert with "[$Hreg $HPC]") as "Hreg";[apply lookup_delete|rewrite insert_delete].
+        
+        iApply wp_value. iIntros (_).
+        iExists _. iFrame. iPureIntro.
+        intros r';simpl. consider_next_reg r' PC. consider_next_reg r' r_t1. consider_next_reg r' r_t2.
+        consider_next_reg r' r_env. consider_next_reg r' r_t0. consider_next_reg r' r_t3. 
+      - (* the shared RO capability *)
+        rewrite decode_encode_perm_inv.
+        rewrite !fixpoint_interp1_eq. iSimpl. apply region_addrs_single in Hincr. rewrite Hincr.
+        iApply big_sepL_singleton. iExists (λne (w : leibnizO Word), ⌜w = inl 1%Z⌝)%I. rewrite /roe_inv. iFrame "Hb".
+        iNext. iAlways. iIntros (w ->). rewrite !fixpoint_interp1_eq. done. 
+      - (* the remaining 0'ed out capabilities *)
+        destruct ((create_gmap_default (map_to_list (delete r_t7 (delete r_t0 rmap))).*1 (inl 0%Z : Word)) !! r) eqn:Hsome;rewrite Hsome.
+        apply create_gmap_default_lookup_is_Some in Hsome as [Hsome ->]. rewrite !fixpoint_interp1_eq. done. rewrite !fixpoint_interp1_eq. done. 
     }
-    iAssert (((interp_reg interp) _ r))%I as "#HvalR";[iSimpl;auto|].
-    iSpecialize ("Hadv_contW''" with "[$HvalR $Hmaps Hsts $Hna $Hr]"); iFrame. 
-    iDestruct "Hadv_contW''" as "[_ Ho]". 
-    rewrite /interp_conf.
-    iApply wp_wand_r. iFrame.
-    iIntros (v) "Htest".
-    iApply "Hφ". 
-    iIntros (->). 
-    iSpecialize ("Htest" with "[]");[auto|]. 
-    iDestruct "Htest" as (r0 W6) "(Hr0 & Hregr0 & % & Hna & Hsts)". 
-    iExists _,_. iFrame.
-    iPureIntro. eapply related_sts_priv_trans_world;[apply HWW''|auto].
+
+    (* conclude that the full program does not get stuck *)
+    iApply (wp_wand with "Hconf");auto. 
   Qed. 
-
-
-End lse.
+    
+End roe. 
