theories/examples/callback.v
@@ -1,0 +1,435 @@
+From iris.algebra Require Import frac.
+From iris.proofmode Require Import tactics.
+Require Import Eqdep_dec List.
+From cap_machine Require Import rules logrel macros_helpers macros call.
+
+Lemma rev_nil_inv {A} (l : list A) :
+  rev l = [] -> l = [].
+Proof.
+  destruct l;auto.
+  simpl. intros Hrev. exfalso.
+  apply app_eq_nil in Hrev as [Hrev1 Hrev2].
+  inversion Hrev2.
+Qed.
+
+Lemma rev_singleton_inv {A} (l : list A) (a : A) :
+  rev l = [a] -> l = [a].
+Proof.
+  destruct l;auto.
+  simpl. intros Hrev.
+  destruct l. 
+  - simpl in Hrev. inversion Hrev. auto. 
+  - exfalso. simpl in Hrev. 
+    apply app_singleton in Hrev. destruct Hrev as [ [Hrev1 Hrev2] | [Hrev1 Hrev2] ].
+    + destruct (rev l);inversion Hrev1. 
+    + inversion Hrev2.
+Qed.
+
+Lemma rev_lookup {A} (l : list A) (a : A) :
+  rev l !! 0 = Some a <-> l !! (length l - 1) = Some a.
+Proof.
+  split; intros Hl.
+  - rewrite -last_lookup.
+    induction l.
+    + inversion Hl.
+    + simpl in Hl. simpl. destruct l.
+      { simpl in Hl. inversion Hl. auto. }
+      { apply IHl. rewrite lookup_app_l in Hl;[|simpl;rewrite app_length /=;lia]. auto. }
+  - rewrite -last_lookup in Hl.
+    induction l.
+    + inversion Hl.
+    + simpl. destruct l.
+      { simpl. inversion Hl. auto. }
+      { rewrite lookup_app_l;[|simpl;rewrite app_length /=;lia]. apply IHl. auto. }
+Qed.
+
+Lemma rev_cons_inv {A} (l l' : list A) (a : A) :
+  rev l = a :: l' ->
+  ∃ l'', l = l'' ++ [a].
+Proof.
+  intros Hrel.
+  destruct l;inversion Hrel.
+  assert ((a0 :: l) !! (length l) = Some a) as Hsome.
+  { assert (length l = length (a0 :: l) - 1) as ->;[simpl;lia|]. apply rev_lookup. rewrite Hrel. constructor. }
+  apply take_S_r in Hsome.
+  exists (take (length l) (rev (rev l ++ [a0]))).
+    simpl. rewrite rev_unit. rewrite rev_involutive. rewrite -Hsome /=. 
+    f_equiv. rewrite firstn_all. auto.
+Qed.     
+
+Section callback.
+  Context {Σ:gFunctors} {memg:memG Σ} {regg:regG Σ}
+          {nainv: logrel_na_invs Σ}
+          `{MP: MachineParameters}.
+
+  (* -------------------------------- LTACS ------------------------------------------- *)
+  
+  (* Tactic for destructing a list into elements *)
+  Ltac destruct_list l :=
+    match goal with
+    | H : strings.length l = _ |- _ =>
+      let a := fresh "a" in
+      let l' := fresh "l" in
+      destruct l as [|a l']; [inversion H|];
+      repeat (let a' := fresh "a" in
+              destruct l' as [|a' l'];[by inversion H|]);
+      destruct l'; [|by inversion H]
+    end.
+
+  Ltac iPrologue_pre :=
+    match goal with
+    | Hlen : length ?a = ?n |- _ =>
+      let a' := fresh "a" in
+      destruct a as [| a' a]; inversion Hlen; simpl
+    end.
+
+  Ltac iPrologue prog :=
+    (try iPrologue_pre);
+    iDestruct prog as "[Hi Hprog]";
+    iApply (wp_bind (fill [SeqCtx])).
+
+  Ltac iEpilogue prog :=
+    iNext; iIntros prog; iSimpl;
+    iApply wp_pure_step_later;auto;iNext.
+
+  Ltac middle_lt prev index :=
+    match goal with
+    | Ha_first : ?a !! 0 = Some ?a_first |- _
+    => apply Z.lt_trans with prev; auto; apply incr_list_lt_succ with a index; auto
+    end.
+
+  Ltac iCorrectPC i j :=
+    eapply isCorrectPC_contiguous_range with (a0 := i) (an := j); eauto; [];
+    cbn; solve [ repeat constructor ].
+
+  Ltac iContiguous_next Ha index :=
+    apply contiguous_of_contiguous_between in Ha;
+    generalize (contiguous_spec _ Ha index); auto.
+
+  Ltac disjoint_from_rmap rmap :=
+    match goal with
+    | Hsub : _ ⊆ dom (gset RegName) rmap |- _ !! ?r = _ => 
+      assert (is_Some (rmap !! r)) as [x Hx];[apply elem_of_gmap_dom;apply Hsub;constructor|];
+      apply map_disjoint_Some_l with rmap x;auto;apply map_disjoint_union_r_2;auto
+    end.
+  
+  Ltac iContiguous_le Ha index :=
+    eapply contiguous_between_middle_bounds with (i:=index) in Ha;eauto;clear -Ha;solve_addr.
+
+  (* ---------------------------------------------------------------------------------- *)
+  
+  Fixpoint restore_locals_instrs r1 locals :=
+    match locals with
+    | [] => []
+    | r :: locals => (lea_z r1 (-1))
+                 :: (load_r r r1)
+                 :: restore_locals_instrs r1 locals
+    end.
+  
+  Definition restore_locals a r1 locals :=
+    ([∗ list] a_i;i ∈ a;(restore_locals_instrs r1 locals), a_i ↦ₐ i)%I.
+
+  Lemma length_restore_locals r1 locals :
+    strings.length (restore_locals_instrs r1 locals) = 2 * length locals. 
+  Proof.
+    induction locals;auto.
+    simpl. lia. 
+  Qed.
+  
+  Lemma restore_locals_spec_middle
+        (* cont *) φ
+        (* list of locals *) r1 locals revlocals mlocals wsr
+        (* PC *) a p b e a_first a_last
+        (* capability for locals *) p_l b_l e_l a_l :
+    isCorrectPC_range p b e a_first a_last →
+    contiguous_between a a_first a_last →
+    region_size b_l a_l = strings.length revlocals →
+    strings.length revlocals > 0 →
+    readAllowed p_l = true → (withinBounds (p_l,b_l,e_l,a_l) = true ∨ a_l = e_l) ->
+    zip locals wsr ≡ₚ(map_to_list mlocals) →
+    length revlocals = length wsr ->
+    rev locals = revlocals ->
+
+    (▷ restore_locals a r1 revlocals
+   ∗ ▷ PC ↦ᵣ inr (p,b,e,a_first)
+   ∗ ▷ r1 ↦ᵣ inr (p_l,b_l,e_l,a_l)
+   ∗ ▷ ([∗ map] r↦_ ∈ mlocals, ∃ w, r ↦ᵣ w)
+   ∗ ▷ ([[b_l,a_l]]↦ₐ[[ wsr ]])
+   ∗ ▷ (PC ↦ᵣ inr (p,b,e,a_last)
+           ∗ r1 ↦ᵣ inr (p_l,b_l,e_l,b_l)
+           ∗ ([∗ map] r↦w ∈ mlocals, r ↦ᵣ w)
+           ∗ [[b_l,a_l]]↦ₐ[[wsr]]
+           ∗ restore_locals a r1 revlocals
+           -∗ WP Seq (Instr Executable) {{ φ }})
+   ⊢ WP Seq (Instr Executable) {{ φ }})%I.
+  Proof.
+    iIntros (Hvpc Hcont Hsize Hnz Hwa Hwb Hperm Hlength Hreveq) "(>Hprog & >HPC& >Hr_t1& >Hlocals& >Hbl& Hcont)".
+    iInduction (revlocals) as [|r revlocals] "IH" forall (a_l mlocals locals wsr a a_first Hreveq Hvpc Hcont Hnz Hsize Hwb Hperm Hlength). 
+    { apply rev_nil_inv in Hreveq as ->. apply Permutation.Permutation_nil in Hperm. inversion Hnz. }
+    destruct revlocals as [|r' revlocals]. 
+    - apply rev_singleton_inv in Hreveq as ->. destruct wsr;[inversion Hlength|]. destruct wsr;[|inversion Hlength]. 
+      apply Permutation_sym, Permutation_singleton in Hperm. 
+      assert (mlocals = {[r:=w]}) as Heq;[|subst mlocals]. 
+      { apply map_to_list_inj. rewrite map_to_list_singleton. apply Permutation_singleton. auto. }
+      rewrite big_sepM_singleton. 
+      rewrite /restore_locals /restore_locals_instrs.
+      iDestruct (big_sepL2_length with "Hbl") as %Hlength_bl.
+      rewrite region_addrs_length Hsize in Hlength_bl.
+      assert (region_addrs b_l a_l = [b_l]) as Heq_locals;[ by rewrite /region_addrs Hsize /=|]. 
+      rewrite /region_mapsto Heq_locals.
+      iDestruct "Hbl" as "[Ha_l _]".
+      iDestruct (big_sepL2_length with "Hprog") as %Hlength_prog.
+      (* lea r_t1 -1 *)
+      destruct_list a.
+      pose proof (contiguous_between_cons_inv_first _ _ _ _ Hcont) as ->. 
+      assert (a_l + (-1) = Some b_l)%a as Hnext.
+      { rewrite /region_size /= in Hsize. revert Hsize;clear;solve_addr. }
+      iPrologue "Hprog". 
+      iApply (wp_lea_success_z with "[$HPC $Hi $Hr_t1]");
+        [apply decode_encode_instrW_inv|iCorrectPC a_first a_last|iContiguous_next Hcont 0|apply Hnext|destruct p_l;auto;inversion Hwa|].
+      iEpilogue "(HPC & Hprog_done & Hr_t1)". 
+      (* load r r_t1 *)
+      pose proof (contiguous_between_last _ _ _ a Hcont eq_refl) as Hlast.
+      iPrologue "Hprog".
+      iDestruct "Hlocals" as (w0) "Hlocals".
+      iAssert (⌜(b_l =? a)%a = false⌝)%I as %Hfalse.
+      { destruct (decide (b_l = a)%Z); [subst|iPureIntro;apply Z.eqb_neq,neq_z_of;auto].
+        iDestruct (mapsto_valid_2 with "Hi Ha_l") as %?. done. }
+      iApply (wp_load_success with "[$HPC $Hi $Hlocals Ha_l $Hr_t1]");
+        [apply decode_encode_instrW_inv|iCorrectPC a_first a_last|split;auto|apply Hlast|..].
+      { revert Hwb. rewrite !andb_true_iff !Z.leb_le !Z.ltb_lt. clear -Hnext. intros [? | Hcontr];[solve_addr|].
+        subst. assert (e_l ≠ b_l) as Hne;[solve_addr|]. solve_addr. }
+      { rewrite Hfalse. iFrame. } rewrite Hfalse. 
+      iEpilogue "(HPC & Hi & Hr & Hr_t1 & Ha_l)".      
+      (* φ *)
+      iApply "Hcont".
+      iFrame. iSplit;[|done]. iApply big_sepM_singleton. iFrame. 
+    - assert (∃ w w0 wsr', wsr = wsr' ++ [w] ++ [w0]) as [w [w0 [wsr' Hwsr'] ] ].
+      { destruct wsr;[inversion Hlength|]. destruct wsr;[inversion Hlength|].
+        destruct wsr.
+        - exists w,w0,[]. auto.
+        - assert (is_Some((w :: w0 :: w1 :: wsr) !! length (w1::wsr))) as [? Hsome]. 
+          { apply lookup_lt_is_Some_2. simpl. lia. }
+          assert (is_Some((w :: w0 :: w1 :: wsr) !! length (w0::w1::wsr))) as [? Hsome']. 
+          { apply lookup_lt_is_Some_2. simpl. lia. }
+          apply take_S_r in Hsome. simpl in Hsome. inversion Hsome.
+          apply take_S_r in Hsome'. simpl in Hsome'. inversion Hsome'.
+          exists x,x0,(take (S(strings.length (wsr))) (w::w0::w1::wsr)). simpl. f_equiv.
+          assert ([x;x0] = [x] ++ [x0]) as ->;auto. rewrite app_assoc -H0. simpl. f_equiv.
+          rewrite -H1. f_equiv. rewrite firstn_all. auto. 
+      }  
+      assert (mlocals !! r = Some w0) as Hrw. 
+      { apply elem_of_map_to_list. rewrite -Hperm.
+        apply rev_cons_inv in Hreveq as Hl''. destruct Hl'' as [l'' Hl'']. 
+        rewrite Hl'' rev_unit in Hreveq. inversion Hreveq.
+        apply rev_cons_inv in H0 as [l3 Hl3]. rewrite Hl3 in Hl''. 
+        rewrite Hl'' Hwsr'. rewrite app_assoc.
+        rewrite zip_app. apply elem_of_app. right. constructor.
+        rewrite !app_length /=. simplify_eq.
+        rewrite -Hreveq /= rev_unit /= !app_length /= rev_length in Hlength. clear -Hlength. lia.  } 
+      iDestruct (big_sepM_delete _ _ r with "Hlocals") as "[Hr Hlocals]";[eauto|]. 
+      assert (is_Some (a_l + (-1))%a) as [a_l' Ha_l'].
+      { rewrite /region_size /= in Hsize. destruct (a_l + -1)%a eqn:Hnone;eauto.
+        simpl in Hsize. revert Hnone Hsize;clear;solve_addr. }
+      assert (region_addrs b_l a_l = region_addrs b_l a_l' ++ [a_l']) as Heq.
+      { rewrite (region_addrs_split _ a_l').
+        assert (region_addrs a_l' a_l = [a_l']) as ->;auto.
+        apply region_addrs_single. clear -Ha_l';solve_addr.
+        rewrite /region_size in Hsize. 
+        clear -Ha_l' Hsize Hwb. solve_addr. }
+      rewrite /region_mapsto Heq.
+      iDestruct "Hr" as (w') "Hr".
+      iDestruct (big_sepL2_length with "Hbl") as %Hlengthbl.
+      rewrite Hwsr'. 
+      rewrite app_assoc. 
+      iDestruct (big_sepL2_app' _ _ _ _ (region_addrs b_l a_l') _ (wsr' ++ [w]) with "Hbl") as "[Hbl Ha_l]".
+      { rewrite Hwsr' in Hlengthbl. rewrite app_length /= app_length /= in Hlengthbl.
+        clear -Hlengthbl. rewrite app_length /=. lia. }
+      iDestruct "Ha_l" as "[Ha_l _]".
+      (* lea r_t1 -1 *)
+      iDestruct (big_sepL2_length with "Hprog") as %Hlength_prog.
+      simpl in Hlength_prog. 
+      destruct a;[inversion Hlength_prog|].
+      destruct a0;[inversion Hlength_prog|]. 
+      pose proof (contiguous_between_cons_inv_first _ _ _ _ Hcont) as ->.
+      iPrologue "Hprog". 
+      iApply (wp_lea_success_z with "[$HPC $Hi $Hr_t1]");
+        [apply decode_encode_instrW_inv|iCorrectPC a_first a_last|iContiguous_next Hcont 0|apply Ha_l'|destruct p_l;auto;inversion Hwa|].
+      iEpilogue "(HPC & Hprog_done & Hr_t1)". 
+      (* load r r_t1 *) simpl in Hlength_prog. 
+      destruct a1;[inversion Hlength_prog|]. 
+      iPrologue "Hprog". 
+      iAssert (⌜(a_l' =? a0)%a = false⌝)%I as %Hfalse.
+      { destruct (decide (a_l' = a0)%Z); [subst|iPureIntro;apply Z.eqb_neq,neq_z_of;auto].
+        iDestruct (mapsto_valid_2 with "Hi Ha_l") as %?. done. }
+      iApply (wp_load_success with "[$HPC $Hi Ha_l $Hr $Hr_t1]");
+        [apply decode_encode_instrW_inv|iCorrectPC a_first a_last|split;auto|iContiguous_next Hcont 1|..].
+      { revert Hwb Hsize. rewrite !andb_true_iff !Z.leb_le !Z.ltb_lt /region_size. clear -Ha_l'.
+        intros [?|Hcontr];[solve_addr|]. subst. assert (e_l ≠ a_l') as Hne;[solve_addr|]. solve_addr. }
+      { rewrite Hfalse. iFrame. } rewrite Hfalse. 
+      iEpilogue "(HPC & Hi & Hr & Hr_t1 & Ha_l)".     
+      apply rev_cons_inv in Hreveq as Hl''. destruct Hl'' as [l'' Hl'']. 
+      iApply ("IH" $! a_l' (delete r mlocals) (l'') (wsr' ++ [w]) with "[] [] [] [] [] [] [] [] Hprog HPC Hr_t1 Hlocals [Hbl]").
+      + iPureIntro. rewrite Hl'' in Hreveq. rewrite rev_unit in Hreveq. inversion Hreveq. auto. 
+      + iPureIntro. eapply isCorrectPC_range_restrict;[eauto|].
+        assert (a_first + 1 = Some a0)%a;[iContiguous_next Hcont 0|].
+        assert (a0 + 1 = Some a)%a;[iContiguous_next Hcont 1|].
+        split;[revert H H0;clear|clear];solve_addr.
+      + iPureIntro.
+        assert (a_first + 1 = Some a0)%a;[iContiguous_next Hcont 0|].
+        assert (a0 + 1 = Some a)%a;[iContiguous_next Hcont 1|].
+        inversion Hcont;simplify_eq.
+        inversion H6;simplify_eq. auto.
+      + iPureIntro;simpl. lia.
+      + iPureIntro. simpl in *.
+        revert Hsize Ha_l'. rewrite /region_size. clear. solve_addr.
+      + iPureIntro. simpl in *.
+        revert Hsize Ha_l' Hwb. rewrite /region_size. clear. intros.
+        destruct Hwb. 
+        ++ left. 
+           apply andb_true_intro. 
+           apply andb_prop in H. revert H. rewrite !Z.leb_le !Z.ltb_lt.
+           intros. 
+           split; try solve_addr.
+        ++ subst. left.
+           apply andb_true_intro.
+           rewrite !Z.leb_le !Z.ltb_lt.
+           intros. 
+           split; try solve_addr.
+      + iPureIntro. rewrite (map_to_list_delete _ _ w0);eauto.
+        rewrite Hl'' rev_unit in Hreveq. inversion Hreveq.
+        apply rev_cons_inv in H0 as [l3 Hl3]. rewrite Hl3. simplify_eq.
+        rewrite -Hperm. rewrite -!app_assoc.
+        assert (length l3 = length wsr') as Hlen.
+        { clear -Hlength Hreveq. rewrite rev_unit in Hreveq. inversion Hreveq. simpl in *.
+          rewrite -rev_length H0. rewrite app_length /= in Hlength. lia. }
+        rewrite !zip_app;auto. rewrite app_assoc. assert (zip [r] [w0] = [(r,w0)]) as ->. auto.
+        rewrite Permutation_cons_append. auto. 
+        rewrite fst_zip Permutation_cons_append. rewrite -Hl''.
+        assert (locals = (zip locals wsr).*1) as ->;[rewrite fst_zip;auto|].
+        { rewrite -rev_length Hreveq. rewrite Hlength. clear;lia. }
+        rewrite Hperm. apply NoDup_map_to_list_fst. apply _. 
+        rewrite app_nil_l app_length /=. rewrite -Hreveq rev_length Hl'' Hwsr' !app_length /= in Hlength. 
+        clear -Hlength. lia. 
+      + rewrite Hl'' rev_unit in Hreveq. inversion Hreveq. rewrite rev_length.
+        apply rev_cons_inv in H0 as [l3 Hl3]. rewrite Hl3. simplify_eq.
+        rewrite rev_unit in Hreveq. inversion Hreveq. simplify_eq.
+        rewrite !app_length /= rev_length in Hlength. 
+        rewrite !app_length /=. iPureIntro. clear -Hlength. lia. 
+      + auto. 
+      + iNext. iIntros "(HPC & Hr_t1 & Hlocals & Hbl & Hprog)".
+        iApply "Hcont". iFrame. iSplit;[|done]. 
+        iApply (big_sepM_delete);[|iFrame]. apply elem_of_map_to_list. rewrite -Hperm.
+        rewrite Hl'' rev_unit in Hreveq. inversion Hreveq.
+        apply rev_cons_inv in H0 as [l3 Hl3]. rewrite Hl3 in Hl''. 
+        rewrite Hl'' Hwsr'. rewrite app_assoc.
+        rewrite zip_app. apply elem_of_app. right. constructor.
+        rewrite !app_length /=. simplify_eq.
+        rewrite -Hreveq /= rev_unit /= !app_length /= rev_length in Hlength. clear -Hlength. lia. 
+  Qed.
+
+
+  Lemma restore_locals_spec
+        (* cont *) φ
+        (* list of locals *) r1 mlocals locals wsr
+        (* PC *) a p b e a_first a_last
+        (* capability for locals *) p_l b_l e_l :
+    isCorrectPC_range p b e a_first a_last →
+    contiguous_between a a_first a_last →
+    region_size b_l e_l = strings.length locals →
+    strings.length locals > 0 → (* we assume the length of locals is non zero, or we would not be able to take a step before invoking continuation *)
+    readAllowed p_l = true →
+    zip locals wsr ≡ₚ(map_to_list mlocals) →
+    length locals = length wsr -> 
+
+    (▷ restore_locals a r1 (rev locals)
+   ∗ ▷ PC ↦ᵣ inr (p,b,e,a_first)
+   ∗ ▷ r1 ↦ᵣ inr (p_l,b_l,e_l,e_l)
+   ∗ ▷ ([∗ map] r↦_ ∈ mlocals, ∃ w, r ↦ᵣ w)
+   ∗ ▷ ([[b_l,e_l]]↦ₐ[[wsr]])
+   ∗ ▷ (PC ↦ᵣ inr (p,b,e,a_last)
+           ∗ r1 ↦ᵣ inr (p_l,b_l,e_l,b_l)
+           ∗ ([∗ map] r↦w ∈ mlocals, r ↦ᵣ w)
+           ∗ [[b_l,e_l]]↦ₐ[[wsr]]
+           ∗ restore_locals a r1 (rev locals)
+           -∗ WP Seq (Instr Executable) {{ φ }})
+   
+   ⊢ WP Seq (Instr Executable) {{ φ }})%I.
+  Proof.
+    iIntros (Hvpc Hcont Hsize Hnz Hwa Hperm Hlen) "(>Hprog & >HPC& >Hr_t1& >Hlocals& >Hbl& Hcont)". 
+    iApply (restore_locals_spec_middle with "[$HPC $Hprog $Hr_t1 $Hlocals $Hbl $Hcont]"); eauto; rewrite rev_length;auto. 
+  Qed.
+
+  Lemma scall_epilogue_spec rt1w rt2w 
+        (* reinstated PC *) pc_p pc_b pc_e a_last a_end
+        (* activation frame *) b_c e_c
+        (* locals *) b_l e_l
+        (* current PC *) p φ :
+
+    isCorrectPC_range p b_c e_c b_c e_c →
+    (a_end + 1)%a = Some a_last ->
+
+    (▷ PC ↦ᵣ inr (p, b_c, e_c, b_c)
+       ∗ ▷ r_t1 ↦ᵣ rt1w
+       ∗ ▷ r_t2 ↦ᵣ rt2w
+       ∗ ▷ ([[b_c,e_c]]↦ₐ[[ [inl hw_1;inl hw_2;inl hw_3;inl hw_4;inl hw_5;inr (RWX,b_l,e_l,e_l);inr (pc_p,pc_b,pc_e,a_end)] ]]) (* activation frame *)
+       ∗ ▷ (PC ↦ᵣ inr (pc_p,pc_b,pc_e,a_last)
+               ∗ (∃ rt1w, r_t1 ↦ᵣ rt1w)
+               ∗ r_t2 ↦ᵣ inr (RWX,b_l,e_l,e_l)
+               ∗ ([[b_c,e_c]]↦ₐ[[ [inl hw_1;inl hw_2;inl hw_3;inl hw_4;inl hw_5;inr (RWX,b_l,e_l,e_l);inr (pc_p,pc_b,pc_e,a_end)] ]]) (* activation frame *) -∗ 
+               WP Seq (Instr Executable) {{ φ }})
+       ⊢ WP Seq (Instr Executable) {{ φ }})%I. 
+  Proof.
+    iIntros (Hvpc Hcontinuation) "(>HPC & >Hr_t1 & >Hr_t2 & >Hprog & Hφ)".
+    iDestruct (big_sepL2_length with "Hprog") as %Hlen.
+    rewrite /= region_addrs_length in Hlen. 
+    assert (b_c <= e_c)%a as Hle.
+    { clear -Hlen. rewrite /region_size in Hlen; solve_addr. }
+    specialize (contiguous_between_region_addrs b_c e_c Hle) as Hcont. 
+    iDestruct (big_sepL2_length with "Hprog") as %Hlength.
+    rewrite /region_mapsto. 
+    destruct (region_addrs b_c e_c);[inversion Hlength|]. 
+    apply contiguous_between_cons_inv_first in Hcont as Heq. subst a. 
+    (* move r_t1 PC *)
+    simpl in Hlength. inversion Hlength. destruct_list l. 
+    iPrologue "Hprog". 
+    iApply (wp_move_success_reg_fromPC with "[$HPC $Hi $Hr_t1]");
+      [apply decode_encode_instrW_inv|iCorrectPC b_c e_c|iContiguous_next Hcont 0|]. 
+    iEpilogue "(HPC & Ha1 & Hr_t1)". 
+    (* lea r_t1 5 *)
+    assert (b_c + 5 = Some a3)%a as Hlea.
+    { apply contiguous_between_incr_addr_middle with (i:=0) (j:=5) (ai:=b_c) (aj:=a3) in Hcont;auto. }
+    iPrologue "Hprog". 
+    iApply (wp_lea_success_z with "[$HPC $Hi $Hr_t1]");
+      [apply decode_encode_instrW_inv|iCorrectPC b_c e_c|iContiguous_next Hcont 1|apply Hlea|..].
+    { eapply isCorrectPC_range_perm_non_E;eauto. rewrite /region_size in Hlen. solve_addr. }
+    iEpilogue "(HPC & Ha2 & Hr_t1)". 
+    (* load r_t2 r_t1 *)
+    iDestruct "Hprog" as "(Ha3 & Ha4 & Ha5 & Ha6 & Ha7 & _)". 
+    iApply (wp_bind (fill [SeqCtx])).
+    iAssert (⌜(a3 =? a0)%a = false⌝)%I as %Hfalse.
+    { destruct (decide (a3 = a0)%Z); [subst|iPureIntro;apply Z.eqb_neq,neq_z_of;auto].
+      iDestruct (mapsto_valid_2 with "Ha3 Ha6") as %?. done. }
+    iApply (wp_load_success with "[$HPC $Ha3 $Hr_t2 $Hr_t1 Ha6]");
+      [apply decode_encode_instrW_inv|iCorrectPC b_c e_c| |iContiguous_next Hcont 2|..].
+    { apply andb_true_iff, Is_true_eq_true. apply isCorrectPC_ra_wb. iCorrectPC b_c e_c. }
+    { rewrite Hfalse. iFrame. }
+    rewrite Hfalse. iEpilogue "(HPC & Hr_t2 & Ha3 & Hr_t1 & Ha6)". 
+    (* lea r_t1 1 *)
+    iApply (wp_bind (fill [SeqCtx])).
+    iApply (wp_lea_success_z with "[$HPC $Ha4 $Hr_t1]");
+      [apply decode_encode_instrW_inv|iCorrectPC b_c e_c|iContiguous_next Hcont 3|iContiguous_next Hcont 5|..].
+    { eapply isCorrectPC_range_perm_non_E;eauto. rewrite /region_size in Hlen. solve_addr. }
+    iEpilogue "(HPC & Ha4 & Hr_t1)". 
+    (* load PC r_t1 *)
+    iApply (wp_bind (fill [SeqCtx])).
+    iApply (wp_load_success_PC with "[$HPC $Ha5 $Hr_t1 $Ha7]");
+      [apply decode_encode_instrW_inv|iCorrectPC b_c e_c| |apply Hcontinuation|..].
+    { apply andb_true_iff, Is_true_eq_true. apply isCorrectPC_ra_wb. iCorrectPC b_c e_c. }
+    iEpilogue "(HPC & Ha5 & Hr_t1 & Ha7)". 
+    (* Hφ *)
+    iApply "Hφ". 
+    iFrame. iSplitL;eauto. 
+  Qed. 
+
+End callback.
