theories/examples/macros.v
@@ -443,8 +443,8 @@ Section macros.
     ([∗ list] a_i;w_i ∈ a;(malloc_instrs f_m size), a_i ↦ₐ w_i)%I. 
 
   (* malloc spec *)
-  Lemma malloc_spec size cont a pc_p pc_b pc_e a_first a_last
-        b_link e_link a_link f_m a_entry mallocN b_m e_m EN rmap φ :
+  Lemma malloc_spec φ size cont a pc_p pc_b pc_e a_first a_last
+        b_link e_link a_link f_m a_entry mallocN b_m e_m EN rmap :
     isCorrectPC_range pc_p pc_b pc_e a_first a_last →
     contiguous_between a a_first a_last →
     withinBounds (RW, b_link, e_link, a_entry) = true →
@@ -614,6 +614,182 @@ Section macros.
     rewrite -(delete_insert_ne _ r_t3) // insert_delete.
     iFrame.
     iExists b,e. iFrame. auto. auto.
+  Qed.
+
+  (* malloc spec - alternative formulation *)
+  Lemma malloc_spec_alt φ ψ size cont a pc_p pc_b pc_e a_first a_last
+        b_link e_link a_link f_m a_entry mallocN b_m e_m EN rmap :
+    isCorrectPC_range pc_p pc_b pc_e a_first a_last →
+    contiguous_between a a_first a_last →
+    withinBounds (RW, b_link, e_link, a_entry) = true →
+    (a_link + f_m)%a = Some a_entry →
+    dom (gset RegName) rmap = all_registers_s ∖ {[ PC; r_t0 ]} →
+    ↑mallocN ⊆ EN →
+    size > 0 →
+
+    (* malloc program and subroutine *)
+    ▷ malloc f_m size a
+    ∗ na_inv logrel_nais mallocN (malloc_inv b_m e_m)
+    ∗ na_own logrel_nais EN
+    (* we need to assume that the malloc capability is in the linking table at offset f_m *)
+    ∗ ▷ pc_b ↦ₐ inr (RO,b_link,e_link,a_link)
+    ∗ ▷ a_entry ↦ₐ inr (E,b_m,e_m,b_m)
+    (* register state *)
+    ∗ ▷ PC ↦ᵣ inr (pc_p,pc_b,pc_e,a_first)
+    ∗ ▷ r_t0 ↦ᵣ cont
+    ∗ ▷ ([∗ map] r_i↦w_i ∈ rmap, r_i ↦ᵣ w_i)
+    (* failure/continuation *)
+    ∗ ▷ (∀ v, ψ v -∗ φ v)
+    ∗ ▷ (ψ FailedV)
+    ∗ ▷ (PC ↦ᵣ inr (pc_p,pc_b,pc_e,a_last) ∗ malloc f_m size a 
+         ∗ pc_b ↦ₐ inr (RO,b_link,e_link,a_link)
+         ∗ a_entry ↦ₐ inr (E,b_m,e_m,b_m)
+         (* the newly allocated region *)
+         ∗ (∃ (b e : Addr),
+            ⌜(b + size)%a = Some e⌝
+            ∗ r_t1 ↦ᵣ inr (RWX,b,e,b)
+            ∗ [[b,e]] ↦ₐ [[region_addrs_zeroes b e]])
+         ∗ r_t0 ↦ᵣ cont
+         ∗ na_own logrel_nais EN
+         ∗ ([∗ map] r_i↦w_i ∈ (<[r_t2:=inl 0%Z]>
+                               (<[r_t3:=inl 0%Z]>
+                                (<[r_t4:=inl 0%Z]>
+                                 (<[r_t5:=inl 0%Z]> (delete r_t1 rmap))))), r_i ↦ᵣ w_i)
+         (* the newly allocated region is fresh in the current world *)
+         (* ∗ ⌜Forall (λ a, a ∉ dom (gset Addr) (std W)) (region_addrs b e)⌝ *)
+         -∗ WP Seq (Instr Executable) {{ ψ }})
+    ⊢
+      WP Seq (Instr Executable) {{ λ v, φ v }}.
+  Proof.
+    iIntros (Hvpc Hcont Hwb Ha_entry Hrmap_dom HmallocN Hsize)
+            "(>Hprog & #Hmalloc & Hna & >Hpc_b & >Ha_entry & >HPC & >Hr_t0 & >Hregs & Hψ & Hφfailed & Hφ)".
+    (* extract necessary registers from regs *)
+    iDestruct (big_sepL2_length with "Hprog") as %Hlength.
+    assert (is_Some (rmap !! r_t1)) as [rv1 ?]. by rewrite elem_of_gmap_dom Hrmap_dom; set_solver.
+    iDestruct (big_sepM_delete _ _ r_t1 with "Hregs") as "[Hr_t1 Hregs]"; eauto.
+    assert (is_Some (rmap !! r_t2)) as [rv2 ?]. by rewrite elem_of_gmap_dom Hrmap_dom; set_solver.
+    iDestruct (big_sepM_delete _ _ r_t2 with "Hregs") as "[Hr_t2 Hregs]". by rewrite lookup_delete_ne //.
+    assert (is_Some (rmap !! r_t3)) as [rv3 ?]. by rewrite elem_of_gmap_dom Hrmap_dom; set_solver.
+    iDestruct (big_sepM_delete _ _ r_t3 with "Hregs") as "[Hr_t3 Hregs]". by rewrite !lookup_delete_ne //.
+    assert (is_Some (rmap !! r_t5)) as [rv5 ?]. by rewrite elem_of_gmap_dom Hrmap_dom; set_solver.
+    iDestruct (big_sepM_delete _ _ r_t5 with "Hregs") as "[Hr_t5 Hregs]". by rewrite !lookup_delete_ne //.
+    destruct a as [|a l];[inversion Hlength|].
+    apply contiguous_between_cons_inv_first in Hcont as Heq. subst.
+    (* fetch f *)
+    iDestruct (contiguous_between_program_split with "Hprog") as (fetch_prog rest link)
+                                                                   "(Hfetch & Hprog & #Hcont)";[apply Hcont|].
+    iDestruct "Hcont" as %(Hcont_fetch & Hcont_rest & Heqapp & Hlink).
+    iApply (fetch_spec with "[- $HPC $Hfetch $Hr_t1 $Hr_t2 $Hr_t3 $Ha_entry $Hpc_b]");
+      [|apply Hcont_fetch|apply Hwb|apply Ha_entry|]. 
+    { intros mid Hmid. apply isCorrectPC_inrange with a_first a_last; auto.
+      apply contiguous_between_bounds in Hcont_rest. revert Hcont_rest Hmid; clear. solve_addr. }
+    iNext. iIntros "(HPC & Hfetch& Hr_t1 & Hr_t2 & Hr_t3 & Hpc_b & Ha_entry)".
+    iDestruct (big_sepL2_length with "Hprog") as %Hlength_rest.
+    assert (isCorrectPC_range pc_p pc_b pc_e link a_last) as Hvpc_rest.
+    { intros mid Hmid. apply isCorrectPC_inrange with a_first a_last; auto. revert Hmid Hlink;clear. solve_addr. }
+    destruct rest as [|a l'];[inversion Hlength_rest|].
+    apply contiguous_between_cons_inv_first in Hcont_rest as Heq. subst.
+    (* move r_t5 r_t0 *)
+    destruct l';[inversion Hlength_rest|]. 
+    iPrologue "Hprog".
+    iApply (wp_move_success_reg with "[$HPC $Hi $Hr_t5 $Hr_t0]");
+      [apply decode_encode_instrW_inv|iCorrectPC link a_last|iContiguous_next Hcont_rest 0|auto|..].
+    iEpilogue "(HPC & Hprog_done & Hr_t5 & Hr_t0)". iCombine "Hprog_done" "Hfetch" as "Hprog_done".
+    (* move r_t3 r_t1 *)
+    destruct l';[inversion Hlength_rest|]. 
+    iPrologue "Hprog".
+    iApply (wp_move_success_reg with "[$HPC $Hi $Hr_t3 $Hr_t1]");
+      [apply decode_encode_instrW_inv|iCorrectPC link a_last|iContiguous_next Hcont_rest 1|auto|..].
+    iEpilogue "(HPC & Hi & Hr_t3 & Hr_t1)"; iCombine "Hi" "Hprog_done" as "Hprog_done".
+    (* move r_t1 size *)
+    destruct l';[inversion Hlength_rest|].
+    iPrologue "Hprog".
+    iApply (wp_move_success_z with "[$HPC $Hi $Hr_t1]");
+      [apply decode_encode_instrW_inv|iCorrectPC link a_last|iContiguous_next Hcont_rest 2|auto|..].
+    iEpilogue "(HPC & Hi & Hr_t1)"; iCombine "Hi" "Hprog_done" as "Hprog_done".
+    (* move r_t0 PC *)
+    destruct l';[inversion Hlength_rest|].
+    iPrologue "Hprog".
+    iApply (wp_move_success_reg_fromPC with "[$HPC $Hi $Hr_t0]");
+      [apply decode_encode_instrW_inv|iCorrectPC link a_last|iContiguous_next Hcont_rest 3|auto|..].
+    iEpilogue "(HPC & Hi & Hr_t0)"; iCombine "Hi" "Hprog_done" as "Hprog_done".
+    (* lea r_t0 3 *)
+    destruct l';[inversion Hlength_rest|]. destruct l';[inversion Hlength_rest|].
+    iPrologue "Hprog".
+    assert ((a1 + 3)%a = Some a4) as Hlea.
+    { apply (contiguous_between_incr_addr_middle _ _ _ 3 3 a1 a4) in Hcont_rest; auto. }
+    iApply (wp_lea_success_z with "[$HPC $Hi $Hr_t0]");
+      [apply decode_encode_instrW_inv|iCorrectPC link a_last|iContiguous_next Hcont_rest 4|apply Hlea|auto..].
+    { apply contiguous_between_length in Hcont.
+      apply isCorrectPC_range_perm in Hvpc; [|revert Hcont; clear; solve_addr].
+      destruct Hvpc as [-> | -> ]; auto. }
+    iEpilogue "(HPC & Hi & Hr_t0)"; iCombine "Hi" "Hprog_done" as "Hprog_done". 
+    (* jmp r_t3 *)
+    destruct l';[inversion Hlength_rest|].
+    iPrologue "Hprog".
+    iApply (wp_jmp_success with "[$HPC $Hi $Hr_t3]");
+      [apply decode_encode_instrW_inv|iCorrectPC link a_last|]. 
+    iEpilogue "(HPC & Hi & Hr_t3) /="; iCombine "Hi" "Hprog_done" as "Hprog_done". 
+    (* we are now ready to use the malloc subroutine spec. For this we prepare the registers *)
+    iDestruct (big_sepM_insert _ _ r_t3 with "[$Hregs $Hr_t3]") as "Hregs".
+      by rewrite lookup_delete_ne // lookup_delete.
+    iDestruct (big_sepM_insert _ _ r_t2 with "[$Hregs $Hr_t2]") as "Hregs".
+      by rewrite lookup_insert_ne // lookup_delete_ne // lookup_delete_ne // lookup_delete.
+    rewrite -(delete_insert_ne _ r_t5 r_t3) // insert_delete.
+    rewrite -(delete_insert_ne _ r_t5 r_t2) // (insert_commute _ r_t2 r_t3) //.
+    rewrite insert_delete.
+    iDestruct (big_sepM_insert _ _ r_t5 with "[$Hregs $Hr_t5]") as "Hregs".
+      by rewrite lookup_delete. rewrite insert_delete.
+    iApply (wp_wand with "[- Hφfailed Hψ]").
+    iApply (simple_malloc_subroutine_spec with "[- $Hmalloc $Hna $Hregs $Hr_t0 $HPC $Hr_t1]"); auto.
+    { rewrite !dom_insert_L dom_delete_L Hrmap_dom.
+      rewrite !difference_difference_L !singleton_union_difference_L !all_registers_union_l.
+      f_equal. set_solver-. }
+    { lia. }
+    iNext.
+    rewrite updatePcPerm_cap_non_E.
+    2: { eapply isCorrectPC_range_perm_non_E; eauto.
+         generalize (contiguous_between_length _ _ _ Hcont_rest). cbn.
+         clear; solve_addr. }
+    iIntros "((Hna & Hregs) & Hr_t0 & HPC & Hbe) /=".
+    iDestruct "Hbe" as (b e Hbe) "(Hr_t1 & Hbe)".
+    iDestruct (big_sepM_delete _ _ r_t3 with "Hregs") as "[Hr_t3 Hregs]".
+      by rewrite lookup_insert_ne // lookup_insert //.
+      rewrite delete_insert_ne // delete_insert_delete.
+      repeat (rewrite delete_insert_ne //;[]). rewrite delete_insert_delete.
+    iDestruct (big_sepM_delete _ _ r_t5 with "Hregs") as "[Hr_t5 Hregs]".
+      by (repeat (rewrite lookup_insert_ne //;[]); rewrite lookup_insert //).
+      repeat (rewrite delete_insert_ne //;[]). rewrite delete_insert_delete.
+    (* move r_t0 r_t5 *)
+    iPrologue "Hprog".
+    iApply (wp_move_success_reg with "[$HPC $Hi $Hr_t0 $Hr_t5]");
+      [apply decode_encode_instrW_inv|iCorrectPC link a_last|iContiguous_next Hcont_rest 6|auto|..].
+    iEpilogue "(HPC & Hi & Hr_t0 & Hr_t5)"; iCombine "Hi" "Hprog_done" as "Hprog_done".
+    (* move r_t5 0 *)
+    destruct l';[| by inversion Hlength_rest].
+    iPrologue "Hprog".
+    apply contiguous_between_last with (ai:=a5) in Hcont_rest as Hlast;[|auto]. 
+    iApply (wp_move_success_z with "[$HPC $Hi $Hr_t5]");
+      [apply decode_encode_instrW_inv|iCorrectPC link a_last|apply Hlast|auto|..].
+    iEpilogue "(HPC & Hi & Hr_t5)"; iCombine "Hi" "Hprog_done" as "Hprog_done".
+    (* continuation *)
+    iApply "Hφ".
+    iFrame "HPC". iSplitL "Hprog_done".
+    { rewrite Heqapp. repeat (iDestruct "Hprog_done" as "[$ Hprog_done]"). iFrame. done. }
+    iFrame.
+    iDestruct (big_sepM_insert _ _ r_t5 with "[$Hregs $Hr_t5]") as "Hregs".
+      repeat (rewrite lookup_insert_ne //;[]). apply lookup_delete.
+    iDestruct (big_sepM_insert _ _ r_t3 with "[$Hregs $Hr_t3]") as "Hregs".
+      repeat (rewrite lookup_insert_ne //;[]).
+      rewrite lookup_delete_ne // lookup_delete //.
+    repeat (rewrite (insert_commute _ r_t5) //;[]).
+    rewrite insert_delete -(delete_insert_ne _ _ r_t5) //.
+    rewrite (insert_commute _ r_t5 r_t2) // (delete_insert_ne _ r_t3 r_t2)//.
+    rewrite (insert_commute _ r_t4 r_t2) // insert_insert.
+    rewrite (insert_commute _ r_t3 r_t2) //.
+    rewrite -(delete_insert_ne _ r_t3) // insert_delete.
+    iFrame.
+    iExists b,e. iFrame. auto. iIntros (v) "[Hφ|Hφ] /=". iApply "Hψ". iFrame. iSimplifyEq. iApply "Hψ". iFrame. 
   Qed.
 
   
